port correctness theorem

Weidenbach_Book/IsaSAT.thy
@@ -696,7 +696,7 @@ lemma init_dt_pre_init:
   by (rule exI[of _ \<open>(([], {#}, {#}, None, {#}, {#}, {#}, {#}), {#})\<close>])
     (auto simp: twl_st_l_init_def twl_init_invs)
       
-lemma
+lemma SAT_l_SAT0:
   assumes dist: \<open>Multiset.Ball (mset `# mset CS) distinct_mset\<close>
   shows \<open>SAT_l CS \<le> \<Down> {(T,T'). (T, T') \<in> twl_st_l None} (SAT0 CS)\<close>
 proof -
@@ -861,18 +861,18 @@ definition (in -) SAT_wl :: \<open>nat clause_l list \<Rightarrow> nat twl_st_wl
           b \<leftarrow> SPEC(\<lambda>_::bool. True);
           if b
           then do {
-             T \<leftarrow> rewatch_st (finalise_init T);
              ASSERT (extract_atms_clss CS {} \<noteq> {});
              ASSERT(isasat_input_bounded_nempty (mset_set \<A>\<^sub>i\<^sub>n'));
              ASSERT(mset `# ran_mf (get_clauses_wl T) + get_unit_clauses_wl T = mset `# mset CS);
              ASSERT(learned_clss_l (get_clauses_wl T) = {#});
+             T \<leftarrow> rewatch_st (finalise_init T);
              cdcl_twl_stgy_restart_prog_wl_D T
           } else do {
-             T \<leftarrow> rewatch_st (finalise_init T);
              ASSERT (extract_atms_clss CS {} \<noteq> {});
              ASSERT(isasat_input_bounded_nempty (mset_set \<A>\<^sub>i\<^sub>n'));
              ASSERT(mset `# ran_mf (get_clauses_wl T) + get_unit_clauses_wl T = mset `# mset CS);
              ASSERT(learned_clss_l (get_clauses_wl T) = {#});
+             T \<leftarrow> rewatch_st (finalise_init T);
              cdcl_twl_stgy_restart_prog_early_wl_D T
           }
         }
@@ -912,18 +912,18 @@ lemma SAT_l_alt_def:
           b \<leftarrow> SPEC(\<lambda>_::bool. True);
           if b
           then do {
-             let T = fst T;
              ASSERT (extract_atms_clss CS {} \<noteq> {});
-	     ASSERT (clauses_to_update_l T = {#});
-             ASSERT(mset `# ran_mf (get_clauses_l T) + get_unit_clauses_l T = mset `# mset CS);
-             ASSERT(learned_clss_l (get_clauses_l T) = {#});
+	     ASSERT (clauses_to_update_l (fst T) = {#});
+             ASSERT(mset `# ran_mf (get_clauses_l (fst T)) + get_unit_clauses_l (fst T) = mset `# mset CS);
+             ASSERT(learned_clss_l (get_clauses_l (fst T)) = {#});
+             let T = fst T;
              cdcl_twl_stgy_restart_prog_l T
           } else do {
-             let T = fst T;
              ASSERT (extract_atms_clss CS {} \<noteq> {});
-	     ASSERT (clauses_to_update_l T = {#});
-             ASSERT(mset `# ran_mf (get_clauses_l T) + get_unit_clauses_l T = mset `# mset CS);
-             ASSERT(learned_clss_l (get_clauses_l T) = {#});
+	     ASSERT (clauses_to_update_l (fst T) = {#});
+             ASSERT(mset `# ran_mf (get_clauses_l (fst T)) + get_unit_clauses_l (fst T) = mset `# mset CS);
+             ASSERT(learned_clss_l (get_clauses_l (fst T)) = {#});
+             let T = fst T;
              cdcl_twl_stgy_restart_prog_early_l T
           }
         }
@@ -1307,28 +1307,7 @@ proof -
          (cdcl_twl_stgy_restart_prog_early_l (fst T'))\<close> (is ?B)
 
     if 
-      \<open>(extract_atms_clss CS {}, \<A>)     \<in> {(x, _). x = extract_atms_clss CS {}}\<close> and
-      \<open>(b, b') \<in> bool_rel\<close> and
-      \<open>(T, \<A>') \<in> init_dt_wl_rel (to_init_state init_state_wl)\<close> and    \<open>(from_init_state T, T')
-       \<in> {(S, S'). S = fst S'} O
-	 {(S, S'). remove_watched S = S'} O state_wl_l_init\<close> and
-      \<open>\<not> get_conflict_wl (from_init_state T) \<noteq> None\<close> and
-      \<open>\<not> get_conflict_l_init T' \<noteq> None\<close> and
-      \<open>CS \<noteq> []\<close> and
-      \<open>CS \<noteq> []\<close> and
-      \<open>(c, c') \<in> bool_rel\<close> and
-      \<open>inres (rewatch_st (finalise_init (from_init_state T))) U'\<close> and
-      U': \<open>(U', fst T') \<in> {(S, T). (S, T) \<in> state_wl_l None \<and> correct_watching S \<and> blits_in_\<L>\<^sub>i\<^sub>n S}\<close> and
-      \<open>extract_atms_clss CS {} \<noteq> {}\<close> and
-      \<open>clauses_to_update_l (fst T') = {#}\<close> and
-      \<open>mset `# ran_mf (get_clauses_l (fst T')) + get_unit_clauses_l (fst T') =
-       mset `# mset CS\<close> and
-      \<open>learned_clss_l (get_clauses_l (fst T')) = {#}\<close> and
-      \<open>extract_atms_clss CS {} \<noteq> {}\<close> and
-      \<open>isasat_input_bounded_nempty (mset_set (extract_atms_clss CS {}))\<close> and
-      \<open>mset `# ran_mf (get_clauses_wl U') + get_unit_clauses_wl U' =
-       mset `# mset CS\<close> and
-      \<open>learned_clss_l (get_clauses_wl U') = {#}\<close>
+      U': \<open>(U', fst T') \<in> {(S, T). (S, T) \<in> state_wl_l None \<and> correct_watching S \<and> blits_in_\<L>\<^sub>i\<^sub>n S}\<close>
       for \<A> b b' T \<A>' T' c c' U'
   proof -
     have 1: \<open> {(T, T'). (T, T') \<in> state_wl_l None} = state_wl_l None\<close>
@@ -1387,33 +1366,25 @@ proof -
     subgoal by auto
     subgoal by (rule conflict_during_init)
     subgoal by auto
-    apply (rule rewatch_st_fst; assumption)
     subgoal using bounded by (auto simp: isasat_input_bounded_nempty_def extract_atms_clss_alt_def
       simp del: isasat_input_bounded_def)
-    subgoal for \<A> b ba T \<A>' T' bb bc U
-     apply (subst (asm) twl_st_wl(2)[of U _ None])
-     apply simp
-     apply (subst (asm) twl_st_wl(10)[of U _ None])
-     apply simp_all
-     done
-    subgoal for \<A> b ba T \<A>' T' bb bc U
-     apply (subst (asm) (2)twl_st_wl(2)[of U _ None])
-     apply simp_all
-     done
+    subgoal for \<A> b ba U \<A>' T' bb bc
+      by (cases U; cases T')
+        (auto simp: state_wl_l_init_def state_wl_l_init'_def)
+    subgoal for \<A> b ba T \<A>' T' bb bc
+      by (auto simp: state_wl_l_init_def state_wl_l_init'_def)
+    apply (rule rewatch_st_fst; assumption)
+
     subgoal by (rule cdcl_twl_stgy_restart_prog_wl_D2)
-    apply (rule rewatch_st_fst; assumption)
+
     subgoal using bounded by (auto simp: isasat_input_bounded_nempty_def extract_atms_clss_alt_def
       simp del: isasat_input_bounded_def)
-    subgoal for \<A> b ba T \<A>' T' bb bc U
-     apply (subst (asm) twl_st_wl(2)[of U _ None])
-     apply simp
-     apply (subst (asm) twl_st_wl(10)[of U _ None])
-     apply simp_all
-     done
-    subgoal for \<A> b ba T \<A>' T' bb bc U
-     apply (subst (asm) (2)twl_st_wl(2)[of U _ None])
-     apply simp_all
-     done
+    subgoal for \<A> b ba U \<A>' T' bb bc
+      by (cases U; cases T')
+        (auto simp: state_wl_l_init_def state_wl_l_init'_def)
+    subgoal for \<A> b ba T \<A>' T' bb bc
+      by (auto simp: state_wl_l_init_def state_wl_l_init'_def)
+    apply (rule rewatch_st_fst; assumption)
     subgoal by (rule cdcl_twl_stgy_restart_prog_early_wl_D2)
     done
 qed
@@ -1456,7 +1427,9 @@ lemma IsaSAT_alt_def:
            ASSERT(isasat_input_bounded_nempty (mset_set \<A>\<^sub>i\<^sub>n'));
            ASSERT(mset `# ran_mf (get_clauses_wl T) + get_unit_clauses_wl T = mset `# mset CS);
            ASSERT(learned_clss_l (get_clauses_wl T) = {#});
-           S \<leftarrow> cdcl_twl_stgy_restart_prog_wl_D (finalise_init T);
+	   _ \<leftarrow> RETURN ();
+	   T \<leftarrow> RETURN (finalise_init T);
+           S \<leftarrow> cdcl_twl_stgy_restart_prog_wl_D (T);
            RETURN (if get_conflict_wl S = None then extract_model_of_state S else extract_stats S)
         }
     }
@@ -1471,19 +1444,23 @@ lemma IsaSAT_alt_def:
           b \<leftarrow> SPEC(\<lambda>_::bool. True);
           if b
           then do {
-             T \<leftarrow> rewatch_st (finalise_init T);
              ASSERT (extract_atms_clss CS {} \<noteq> {});
              ASSERT(isasat_input_bounded_nempty (mset_set \<A>\<^sub>i\<^sub>n'));
              ASSERT(mset `# ran_mf (get_clauses_wl T) + get_unit_clauses_wl T = mset `# mset CS);
              ASSERT(learned_clss_l (get_clauses_wl T) = {#});
-             S \<leftarrow> cdcl_twl_stgy_restart_prog_wl_D T;
+             _ \<leftarrow> RETURN ();
+             T \<leftarrow> rewatch_st T;
+	     T \<leftarrow> RETURN (finalise_init T);
+	     S \<leftarrow> cdcl_twl_stgy_restart_prog_wl_D T;
              RETURN (if get_conflict_wl S = None then extract_model_of_state S else extract_stats S)
           } else do {
-             T \<leftarrow> rewatch_st (finalise_init T);
              ASSERT (extract_atms_clss CS {} \<noteq> {});
              ASSERT(isasat_input_bounded_nempty (mset_set \<A>\<^sub>i\<^sub>n'));
              ASSERT(mset `# ran_mf (get_clauses_wl T) + get_unit_clauses_wl T = mset `# mset CS);
              ASSERT(learned_clss_l (get_clauses_wl T) = {#});
+             _ \<leftarrow> RETURN ();
+             T \<leftarrow> rewatch_st T;
+	     T \<leftarrow> RETURN (finalise_init T);
              S \<leftarrow> cdcl_twl_stgy_restart_prog_early_wl_D T;
              RETURN (if get_conflict_wl S = None then extract_model_of_state S else extract_stats S)
           }
@@ -1495,7 +1472,7 @@ proof -
     by auto
   have 1: \<open>?A \<le> \<Down> Id ?B\<close>
     unfolding IsaSAT_def SAT_wl_def nres_bind_let_law If_bind_distrib nres_monad_laws
-      Let_def
+      Let_def finalise_init_def
     apply (refine_vcg)
     subgoal by auto
     apply (rule H; solves auto)
@@ -1513,21 +1490,21 @@ proof -
     subgoal by auto
     subgoal by (auto simp: extract_model_of_state_def)
     subgoal by auto
-    apply (rule H; solves auto)
     subgoal by auto
     subgoal by auto
     apply (rule H; solves auto)
-    subgoal by auto
     apply (rule H; solves auto)
     subgoal by auto
     subgoal by auto
+    subgoal by auto
+    apply (rule H; solves auto)
     apply (rule H; solves auto)
     subgoal by auto
     done
 
   have 2: \<open>?B \<le> \<Down> Id ?A\<close>
     unfolding IsaSAT_def SAT_wl_def nres_bind_let_law If_bind_distrib nres_monad_laws
-      Let_def
+      Let_def finalise_init_def
     apply (refine_vcg)
     subgoal by auto
     apply (rule H; solves auto)
@@ -1545,14 +1522,14 @@ proof -
     subgoal by auto
     subgoal by (auto simp: extract_model_of_state_def)
     subgoal by auto
-    apply (rule H; solves auto)
     subgoal by auto
     subgoal by auto
     apply (rule H; solves auto)
-    subgoal by auto
     apply (rule H; solves auto)
     subgoal by auto
     subgoal by auto
+    subgoal by auto
+    apply (rule H; solves auto)
     apply (rule H; solves auto)
     subgoal by auto
     done
@@ -1640,6 +1617,9 @@ lemma isasat_init_fast_slow_alt_def:
     convert_wlists_to_nat_conv_def
   by auto
 
+definition isasat_fast_init :: \<open>twl_st_wl_heur_init \<Rightarrow> bool\<close> where
+  \<open>isasat_fast_init S \<longleftrightarrow> (length (get_clauses_wl_heur_init S) \<le> uint64_max - (uint32_max + 5))\<close>
+
 definition IsaSAT_heur :: \<open>opts \<Rightarrow> nat clause_l list \<Rightarrow> (nat literal list option \<times> stats) nres\<close> where
   \<open>IsaSAT_heur opts CS = do{
     ASSERT(isasat_input_bounded (mset_set (extract_atms_clss CS {})));
@@ -1679,8 +1659,21 @@ definition IsaSAT_heur :: \<open>opts \<Rightarrow> nat clause_l list \<Rightarr
         then RETURN (empty_init_code)
         else if CS = [] then empty_conflict_code
         else 
-          if length (get_clauses_wl_heur_init T) \<le> uint64_max
-          then do {
+          if \<not>(isasat_fast_init T)
+         then do {
+           ASSERT(\<A>\<^sub>i\<^sub>n'' \<noteq> {#});
+           ASSERT(isasat_input_bounded_nempty \<A>\<^sub>i\<^sub>n'');
+           _ \<leftarrow> isasat_information_banner T;
+           ASSERT((\<lambda>(M', N', D', Q', W', ((ns, m, fst_As, lst_As, next_search), to_remove), \<phi>, clvls). fst_As \<noteq> None \<and>
+             lst_As \<noteq> None) T);
+	   T \<leftarrow> isasat_init_fast_slow T;
+	   T \<leftarrow> rewatch_heur_st T;
+           T \<leftarrow> finalise_init_code opts (T::twl_st_wl_heur_init);
+           U \<leftarrow> cdcl_twl_stgy_restart_prog_wl_heur T;
+           RETURN (if get_conflict_wl_is_None_heur U then extract_model_of_state_stat U
+             else extract_state_stat U)
+         }
+         else do {
            ASSERT(\<A>\<^sub>i\<^sub>n'' \<noteq> {#});
            ASSERT(isasat_input_bounded_nempty \<A>\<^sub>i\<^sub>n'');
            _ \<leftarrow> isasat_information_banner T;
@@ -1691,19 +1684,6 @@ definition IsaSAT_heur :: \<open>opts \<Rightarrow> nat clause_l list \<Rightarr
            T \<leftarrow> finalise_init_code opts (T::twl_st_wl_heur_init);
 	   ASSERT(isasat_fast T);
            U \<leftarrow> cdcl_twl_stgy_restart_prog_early_wl_heur T;
-           RETURN (if get_conflict_wl_is_None_heur U then extract_model_of_state_stat U
-             else extract_state_stat U)
-         }
-         else do {
-           ASSERT(\<A>\<^sub>i\<^sub>n'' \<noteq> {#});
-           ASSERT(isasat_input_bounded_nempty \<A>\<^sub>i\<^sub>n'');
-           _ \<leftarrow> isasat_information_banner T;
-           ASSERT((\<lambda>(M', N', D', Q', W', ((ns, m, fst_As, lst_As, next_search), to_remove), \<phi>, clvls). fst_As \<noteq> None \<and>
-             lst_As \<noteq> None) T);
-	   T \<leftarrow> isasat_init_fast_slow T;
-	   T \<leftarrow> rewatch_heur_st T;
-           T \<leftarrow> finalise_init_code opts (T::twl_st_wl_heur_init);
-           U \<leftarrow> cdcl_twl_stgy_restart_prog_wl_heur T;
            RETURN (if get_conflict_wl_is_None_heur U then extract_model_of_state_stat U
              else extract_state_stat U)
          }
@@ -1722,6 +1702,46 @@ proof -
     by (auto simp: conc_fun_RES Image_iff)
 qed
 
+lemma fref_to_Down_unRET_SPEC:
+  assumes \<open>(f, RETURN o g) \<in> [P]\<^sub>f A \<rightarrow> \<langle>B\<rangle>nres_rel\<close> and
+    \<open>P y\<close> and
+    \<open>(x, y) \<in> A\<close>
+  shows \<open>f x \<le> SPEC (\<lambda>c. (c, g y) \<in> B)\<close>
+proof -
+  have [simp]: \<open>RES (B\<inverse> `` {g}) = SPEC (\<lambda>c. (c, g) \<in> B)\<close> for g
+    by auto
+  show ?thesis
+    using assms
+    unfolding fref_def uncurry_def nres_rel_def RETURN_def
+    by (auto simp: conc_fun_RES Image_iff)
+qed
+
+lemma fref_to_Down_unRET_curry_SPEC:
+  assumes \<open>(uncurry f, uncurry (RETURN oo g)) \<in> [P]\<^sub>f A \<rightarrow> \<langle>B\<rangle>nres_rel\<close> and
+    \<open>P (x, y)\<close> and
+    \<open>((x', y'), (x, y)) \<in> A\<close>
+  shows \<open>f x' y' \<le> SPEC (\<lambda>c. (c, g x y) \<in> B)\<close>
+proof -
+  have [simp]: \<open>RES (B\<inverse> `` {g}) = SPEC (\<lambda>c. (c, g) \<in> B)\<close> for g
+    by auto
+  show ?thesis
+    using assms
+    unfolding fref_def uncurry_def nres_rel_def RETURN_def
+    by (auto simp: conc_fun_RES Image_iff)
+qed
+
+lemma all_lits_of_mm_empty_iff: \<open>all_lits_of_mm A = {#} \<longleftrightarrow> (\<forall>C \<in># A. C = {#})\<close>
+  apply (induction A)
+  subgoal by auto
+  subgoal by (auto simp: all_lits_of_mm_add_mset)
+  done
+
+lemma all_lits_of_mm_extract_atms_clss:
+  \<open>L \<in># (all_lits_of_mm (mset `# mset CS)) \<longleftrightarrow> atm_of L \<in> extract_atms_clss CS {}\<close>
+  by (induction CS)
+    (auto simp: extract_atms_clss_alt_def all_lits_of_mm_add_mset
+    in_all_lits_of_m_ain_atms_of_iff)
+  
 lemma IsaSAT_heur_alt_def:
   \<open>IsaSAT_heur opts CS = do{
     ASSERT(isasat_input_bounded (mset_set (extract_atms_clss CS {})));
@@ -1759,40 +1779,135 @@ lemma IsaSAT_heur_alt_def:
         if \<not>get_conflict_wl_is_None_heur_init T
         then RETURN (empty_init_code)
         else if CS = [] then empty_conflict_code
-        else 
-          if length (get_clauses_wl_heur_init T) \<le> uint64_max
+        else
+	  let b = \<not>isasat_fast_init T in
+          if b
           then do {
            ASSERT(\<A>\<^sub>i\<^sub>n'' \<noteq> {#});
-           ASSERT(isasat_input_bounded_nempty \<A>\<^sub>i\<^sub>n'');
-           _ \<leftarrow> isasat_information_banner T;
-           ASSERT((\<lambda>(M', N', D', Q', W', ((ns, m, fst_As, lst_As, next_search), to_remove), \<phi>, clvls). fst_As \<noteq> None \<and>
-             lst_As \<noteq> None) T);
-	   ASSERT(rewatch_heur_st_fast_pre T);
-	   T \<leftarrow> rewatch_heur_st_fast T;
-           T \<leftarrow> finalise_init_code opts (T::twl_st_wl_heur_init);
-	   ASSERT(isasat_fast T);
-           U \<leftarrow> cdcl_twl_stgy_restart_prog_early_wl_heur T;
-           RETURN (if get_conflict_wl_is_None_heur U then extract_model_of_state_stat U
-             else extract_state_stat U)
-         }
-         else do {
-           ASSERT(\<A>\<^sub>i\<^sub>n'' \<noteq> {#});
-           ASSERT(isasat_input_bounded_nempty \<A>\<^sub>i\<^sub>n'');
-           _ \<leftarrow> isasat_information_banner T;
-           ASSERT((\<lambda>(M', N', D', Q', W', ((ns, m, fst_As, lst_As, next_search), to_remove), \<phi>, clvls). fst_As \<noteq> None \<and>
-             lst_As \<noteq> None) T);
-	   T \<leftarrow> rewatch_heur_st T;
-           T \<leftarrow> finalise_init_code opts (T::twl_st_wl_heur_init);
-           U \<leftarrow> cdcl_twl_stgy_restart_prog_wl_heur T;
-           RETURN (if get_conflict_wl_is_None_heur U then extract_model_of_state_stat U
-             else extract_state_stat U)
-         }
+	    ASSERT(isasat_input_bounded_nempty \<A>\<^sub>i\<^sub>n'');
+	    _ \<leftarrow> isasat_information_banner T;
+	    ASSERT((\<lambda>(M', N', D', Q', W', ((ns, m, fst_As, lst_As, next_search), to_remove), \<phi>, clvls). fst_As \<noteq> None \<and>
+	      lst_As \<noteq> None) T);
+	    T \<leftarrow> rewatch_heur_st T;
+	    T \<leftarrow> finalise_init_code opts (T::twl_st_wl_heur_init);
+	    U \<leftarrow> cdcl_twl_stgy_restart_prog_wl_heur T;
+	    RETURN (if get_conflict_wl_is_None_heur U then extract_model_of_state_stat U
+	      else extract_state_stat U)
+	  }
+	  else do {
+	    ASSERT(\<A>\<^sub>i\<^sub>n'' \<noteq> {#});
+	    ASSERT(isasat_input_bounded_nempty \<A>\<^sub>i\<^sub>n'');
+	    _ \<leftarrow> isasat_information_banner T;
+	    ASSERT((\<lambda>(M', N', D', Q', W', ((ns, m, fst_As, lst_As, next_search), to_remove), \<phi>, clvls). fst_As \<noteq> None \<and>
+	      lst_As \<noteq> None) T);
+	    ASSERT(rewatch_heur_st_fast_pre T);
+	    T \<leftarrow> rewatch_heur_st_fast T;
+	    T \<leftarrow> finalise_init_code opts (T::twl_st_wl_heur_init);
+	    ASSERT(isasat_fast T);
+	    U \<leftarrow> cdcl_twl_stgy_restart_prog_early_wl_heur T;
+	    RETURN (if get_conflict_wl_is_None_heur U then extract_model_of_state_stat U
+	      else extract_state_stat U)
+	  }
       }
     }\<close>
   by (auto simp: IsaSAT_heur_def isasat_init_fast_slow_alt_def cong: if_cong)
 
-lemma
-  \<open>IsaSAT_heur b CS \<le> \<Down>{((M, stats), M'). M = M'} (IsaSAT CS)\<close>
+(*TODO Move*)
+lemma Collect_eq_comp': \<open> {(x, y). P x y} O {(c, a). c = f a} = {(x, a). P x (f a)}\<close>
+  by auto
+(*End Move*)
+
+lemma rewatch_heur_st_rewatch_st:
+  assumes 
+    UV: \<open>(U, V)
+     \<in> twl_st_heur_parsing_no_WL (mset_set (extract_atms_clss CS {})) O
+       {(S, T). S = remove_watched T \<and> get_watched_wl (fst T) = (\<lambda>_. [])}\<close>
+  shows \<open>rewatch_heur_st U \<le>
+    \<Down>({(S,T). (S, T) \<in> twl_st_heur_parsing (mset_set (extract_atms_clss CS {})) \<and>
+         get_clauses_wl_heur_init S = get_clauses_wl_heur_init U \<and>
+	 get_conflict_wl_heur_init S = get_conflict_wl_heur_init U \<and>
+         get_clauses_wl (fst T) = get_clauses_wl (fst V) \<and>
+	 get_conflict_wl (fst T) = get_conflict_wl (fst V) \<and>
+	 get_unit_clauses_wl (fst T) = get_unit_clauses_wl (fst V)} O {(S, T). S = (T, {#})})
+           (rewatch_st (from_init_state V))\<close>
+proof -
+  let ?\<A> = \<open>(mset_set (extract_atms_clss CS {}))\<close>
+  obtain M' arena D' j W' vm \<phi> clvls cach lbd vdom M N D NE UE Q W OC where
+    U: \<open>U = ((M', arena, D', j, W', vm, \<phi>, clvls, cach, lbd, vdom))\<close> and
+    V: \<open>V = ((M, N, D, NE, UE, Q, W), OC)\<close>
+    by (cases U; cases V) auto
+  have valid: \<open>valid_arena arena N (set vdom)\<close> and
+    dist: \<open>distinct vdom\<close> and
+    vdom_N: \<open>mset vdom = dom_m N\<close> and
+    watched: \<open>(W', W) \<in> \<langle>Id\<rangle>map_fun_rel (D\<^sub>0 ?\<A>)\<close> and
+    lall: \<open>literals_are_in_\<L>\<^sub>i\<^sub>n_mm ?\<A> (mset `# ran_mf N)\<close> and
+    vdom: \<open>vdom_m ?\<A> W N \<subseteq> set_mset (dom_m N)\<close>
+    using UV by (auto simp: twl_st_heur_parsing_no_WL_def U V distinct_mset_dom
+      empty_watched_def vdom_m_def literals_are_in_\<L>\<^sub>i\<^sub>n_mm_def
+      all_lits_of_mm_union
+      simp flip: distinct_mset_mset_distinct)
+
+  show ?thesis
+    using UV
+    unfolding rewatch_heur_st_def rewatch_st_def
+    apply (simp only: prod.simps from_init_state_def fst_conv nres_monad1 U V)
+    apply refine_vcg
+    apply (rule rewatch_heur_rewatch[OF valid _ dist _ watched lall])
+    subgoal by simp
+    subgoal using vdom_N[symmetric] by simp
+    subgoal by (auto simp: vdom_m_def)
+    subgoal by (auto simp: U V twl_st_heur_parsing_def Collect_eq_comp'
+      twl_st_heur_parsing_no_WL_def)
+    done
+qed
+
+lemma rewatch_heur_st_rewatch_st2:
+  assumes
+    T: \<open>(U, V)
+     \<in> twl_st_heur_parsing_no_WL (mset_set (extract_atms_clss CS {})) O
+       {(S, T). S = remove_watched T \<and> get_watched_wl (fst T) = (\<lambda>_. [])}\<close>
+  shows \<open>rewatch_heur_st_fast
+          (convert_state (virtual_copy (mset_set (extract_atms_clss CS {}))) U)
+         \<le> \<Down> ({(S,T). (S, T) \<in> twl_st_heur_parsing (mset_set (extract_atms_clss CS {})) \<and>
+         get_clauses_wl_heur_init S = get_clauses_wl_heur_init U \<and>
+	 get_conflict_wl_heur_init S = get_conflict_wl_heur_init U \<and>
+         get_clauses_wl (fst T) = get_clauses_wl (fst V) \<and>
+	 get_conflict_wl (fst T) = get_conflict_wl (fst V) \<and>
+	 get_unit_clauses_wl (fst T) = get_unit_clauses_wl (fst V)} O {(S, T). S = (T, {#})})
+            (rewatch_st (from_init_state V))\<close>
+proof -
+  have
+    UV: \<open>(U, V)
+     \<in> twl_st_heur_parsing_no_WL (mset_set (extract_atms_clss CS {})) O
+       {(S, T). S = remove_watched T \<and> get_watched_wl (fst T) = (\<lambda>_. [])}\<close>
+    using T by (auto simp: twl_st_heur_parsing_no_WL_def)
+  then show ?thesis
+    unfolding convert_state_def finalise_init_def id_def rewatch_heur_st_fast_def
+    by (rule rewatch_heur_st_rewatch_st[of U V, THEN order_trans])
+      (auto intro!: conc_fun_R_mono simp: Collect_eq_comp'
+        twl_st_heur_parsing_def)
+qed
+
+(*TODO Move*)
+  
+lemma vmtf_init_cong:
+  \<open>set_mset \<A> = set_mset \<B> \<Longrightarrow> L \<in> vmtf_init \<A> M \<Longrightarrow> L \<in> vmtf_init \<B> M\<close>
+  using \<L>\<^sub>a\<^sub>l\<^sub>l_cong[of \<A> \<B>] atms_of_\<L>\<^sub>a\<^sub>l\<^sub>l_cong[of \<A> \<B>] vmtf_cong[of \<A> \<B>]
+  unfolding vmtf_init_def vmtf_\<L>\<^sub>a\<^sub>l\<^sub>l_def
+  by (auto simp: )
+
+lemma isa_vmtf_init_cong:
+  \<open>set_mset \<A> = set_mset \<B> \<Longrightarrow> L \<in> isa_vmtf_init \<A> M \<Longrightarrow> L \<in> isa_vmtf_init \<B> M\<close>
+  using vmtf_init_cong[of \<A> \<B>]  distinct_atoms_rel_cong[of \<A> \<B>]
+  apply (subst (asm) isa_vmtf_init_def)
+  apply (cases L)
+  by (auto intro!: isa_vmtf_initI)
+
+lemma finite_extract_atms_clss[simp]: \<open>finite (extract_atms_clss CS' {})\<close> for CS'
+  by (auto simp: extract_atms_clss_alt_def)
+
+lemma IsaSAT_heur_IsaSAT:
+  \<open>IsaSAT_heur b CS \<le> \<Down>{((M, stats), M'). M = map_option rev M'} (IsaSAT CS)\<close>
 proof -
   have init_dt_wl_heur: \<open>init_dt_wl_heur CS S \<le>
        \<Down>(twl_st_heur_parsing_no_WL \<A> O {(S, T). S = remove_watched T \<and>
@@ -1843,10 +1958,297 @@ proof -
     apply (auto)
     done
 
+  have get_conflict_wl_is_None_heur_init: \<open> (Tb, Tc)
+    \<in> ({(S,T). (S, T) \<in> twl_st_heur_parsing (mset_set (extract_atms_clss CS {})) \<and>
+         get_clauses_wl_heur_init S = get_clauses_wl_heur_init U \<and>
+	 get_conflict_wl_heur_init S = get_conflict_wl_heur_init U \<and>
+         get_clauses_wl (fst T) = get_clauses_wl (fst V) \<and>
+	 get_conflict_wl (fst T) = get_conflict_wl (fst V) \<and>
+	 get_unit_clauses_wl (fst T) = get_unit_clauses_wl (fst V)} O {(S, T). S = (T, {#})}) \<Longrightarrow>
+    (\<not> get_conflict_wl_is_None_heur_init Tb) = (get_conflict_wl Tc \<noteq> None)\<close> for Tb Tc U V
+    by (cases V) (auto simp: twl_st_heur_parsing_def Collect_eq_comp'
+      get_conflict_wl_is_None_heur_init_def
+      option_lookup_clause_rel_def)
 
+  have finalise_init_nempty: \<open>x1i \<noteq> None\<close> \<open>x1j \<noteq> None\<close>
+    if 
+      T: \<open>(Tb, Tc)
+       \<in> ({(S,T). (S, T) \<in> twl_st_heur_parsing (mset_set (extract_atms_clss CS {})) \<and>
+         get_clauses_wl_heur_init S = get_clauses_wl_heur_init U \<and>
+	 get_conflict_wl_heur_init S = get_conflict_wl_heur_init U \<and>
+         get_clauses_wl (fst T) = get_clauses_wl (fst V) \<and>
+	 get_conflict_wl (fst T) = get_conflict_wl (fst V) \<and>
+	 get_unit_clauses_wl (fst T) = get_unit_clauses_wl (fst V)} O {(S, T). S = (T, {#})})\<close> and
+      nempty: \<open>extract_atms_clss CS {} \<noteq> {}\<close> and
+      st:
+        \<open>x2g = (x1j, x2h)\<close> 
+	\<open>x2f = (x1i, x2g)\<close> 
+	\<open>x2e = (x1h, x2f)\<close> 
+	\<open>x1f = (x1g, x2e)\<close> 
+	\<open>x1e = (x1f, x2i)\<close> 
+	\<open>x2j = (x1k, x2k)\<close> 
+	\<open>x2d = (x1e, x2j)\<close> 
+	\<open>x2c = (x1d, x2d)\<close> 
+	\<open>x2b = (x1c, x2c)\<close> 
+	\<open>x2a = (x1b, x2b)\<close> 
+	\<open>x2 = (x1a, x2a)\<close> and
+      conv: \<open>convert_state (virtual_copy (mset_set (extract_atms_clss CS {}))) Tb =
+       (x1, x2)\<close>
+    for ba S T Ta Tb Tc uu x1 x2 x1a x2a x1b x2b x1c x2c x1d x2d x1e x1f
+      x1g x2e x1h x2f x1i x2g x1j x2h x2i x2j x1k x2k U V
+  proof -
+    show \<open>x1i \<noteq> None\<close> 
+      using T conv nempty
+      unfolding st
+      by (cases x1i)
+       (auto simp: convert_state_def twl_st_heur_parsing_def
+        isa_vmtf_init_def vmtf_init_def mset_set_empty_iff)
+    show \<open>x1j \<noteq> None\<close> 
+      using T conv nempty
+      unfolding st
+      by (cases x1i)
+       (auto simp: convert_state_def twl_st_heur_parsing_def
+        isa_vmtf_init_def vmtf_init_def mset_set_empty_iff)
+  qed
+
+  have banner: \<open>isasat_information_banner
+     (convert_state (virtual_copy (mset_set (extract_atms_clss CS {}))) Tb)
+    \<le> SPEC (\<lambda>c. (c, ()) \<in> {(_, _). True})\<close> for Tb
+    by (auto simp: isasat_information_banner_def)
+
+  have finalise_init_code: \<open>finalise_init_code b
+	 (convert_state (virtual_copy (mset_set (extract_atms_clss CS {}))) Tb)
+	\<le> SPEC (\<lambda>c. (c, finalise_init Tc) \<in> twl_st_heur)\<close>
+    if 
+      T: \<open>(Tb, Tc)
+       \<in> ({(S,T). (S, T) \<in> twl_st_heur_parsing (mset_set (extract_atms_clss CS {})) \<and>
+         get_clauses_wl_heur_init S = get_clauses_wl_heur_init U \<and>
+	 get_conflict_wl_heur_init S = get_conflict_wl_heur_init U \<and>
+         get_clauses_wl (fst T) = get_clauses_wl (fst V) \<and>
+	 get_conflict_wl (fst T) = get_conflict_wl (fst V) \<and>
+	 get_unit_clauses_wl (fst T) = get_unit_clauses_wl (fst V)} O {(S, T). S = (T, {#})})\<close> and
+      confl: \<open>\<not> get_conflict_wl Tc \<noteq> None\<close> and
+      nempty: \<open>extract_atms_clss CS {} \<noteq> {}\<close> and
+      clss_CS: \<open>mset `# ran_mf (get_clauses_wl Tc) + get_unit_clauses_wl Tc =
+       mset `# mset CS\<close> and
+      learned: \<open>learned_clss_l (get_clauses_wl Tc) = {#}\<close>
+    for ba S T Ta Tb Tc u v U V
+  proof -
+    have 1: \<open>get_conflict_wl Tc = None\<close>
+      using confl by auto
+    have 2: \<open>all_atms (get_clauses_wl Tc) (get_unit_clauses_wl Tc) \<noteq> {#}\<close>
+      using clss_CS nempty
+      by (auto simp flip: all_atms_def[symmetric] simp: all_lits_def
+        isasat_input_bounded_nempty_def extract_atms_clss_alt_def
+	all_lits_of_mm_empty_iff)
+    have 3: \<open>set_mset (all_atms_st Tc) = set_mset (mset_set (extract_atms_clss CS {}))\<close>
+      using clss_CS nempty
+      by (auto simp flip: all_atms_def[symmetric] simp: all_lits_def
+        isasat_input_bounded_nempty_def
+  	atm_of_all_lits_of_mm extract_atms_clss_alt_def atms_of_ms_def)
+    have H: \<open>A = B \<Longrightarrow> x \<in> A \<Longrightarrow> x \<in> B\<close> for A B x
+      by auto
+    have H': \<open>A = B \<Longrightarrow> A x \<Longrightarrow> B x\<close> for A B x
+      by auto
+
+    note cong =  trail_pol_cong
+      option_lookup_clause_rel_cong isa_vmtf_init_cong
+       vdom_m_cong[THEN H] isasat_input_nempty_cong[THEN iffD1]
+      isasat_input_bounded_cong[THEN iffD1]
+       cach_refinement_empty_cong[THEN H']
+       phase_saving_cong[THEN H']
+       \<L>\<^sub>a\<^sub>l\<^sub>l_cong[THEN H]
+       D\<^sub>0_cong[THEN H]
+
+    have 4: \<open>(convert_state (mset_set (extract_atms_clss CS {})) Tb, Tc)
+    \<in> twl_st_heur_post_parsing_wl\<close>
+      using T  nempty
+      by (auto simp: twl_st_heur_parsing_def twl_st_heur_post_parsing_wl_def
+        convert_state_def eq_commute[of \<open>mset _\<close> \<open>dom_m _\<close>]
+	vdom_m_cong[OF 3[symmetric]] \<L>\<^sub>a\<^sub>l\<^sub>l_cong[OF 3[symmetric]]
+	dest!: cong[OF 3[symmetric]])
+    show ?thesis
+     by (rule finalise_init_finalise_init[THEN fref_to_Down_unRET_curry_SPEC, of b])
+      (use 1 2 learned 4 in auto)
+  qed
+
+  have get_conflict_wl_is_None_heur_init2: \<open>(U, V)
+    \<in> twl_st_heur_parsing_no_WL (mset_set (extract_atms_clss CS {})) O
+      {(S, T). S = remove_watched T \<and> get_watched_wl (fst T) = (\<lambda>_. [])} \<Longrightarrow>
+    (\<not> get_conflict_wl_is_None_heur_init
+        (convert_state (virtual_copy (mset_set (extract_atms_clss CS {}))) U)) =
+    (get_conflict_wl (from_init_state V) \<noteq> None)\<close> for U V
+    by (auto simp: twl_st_heur_parsing_def Collect_eq_comp'
+      get_conflict_wl_is_None_heur_init_def twl_st_heur_parsing_no_WL_def
+      option_lookup_clause_rel_def convert_state_def from_init_state_def)
+
+  have finalise_init2:  \<open>x1i \<noteq> None\<close> \<open>x1j \<noteq> None\<close>
+    if 
+      T: \<open>(T, Ta)
+       \<in> twl_st_heur_parsing_no_WL (mset_set (extract_atms_clss CS {})) O
+	 {(S, T). S = remove_watched T \<and> get_watched_wl (fst T) = (\<lambda>_. [])}\<close> and
+      nempty: \<open>extract_atms_clss CS {} \<noteq> {}\<close> and
+      st:
+        \<open>x2g = (x1j, x2h)\<close>
+	\<open>x2f = (x1i, x2g)\<close>
+	\<open>x2e = (x1h, x2f)\<close>
+	\<open>x1f = (x1g, x2e)\<close>
+	\<open>x1e = (x1f, x2i)\<close>
+	\<open>x2j = (x1k, x2k)\<close>
+	\<open>x2d = (x1e, x2j)\<close>
+	\<open>x2c = (x1d, x2d)\<close>
+	\<open>x2b = (x1c, x2c)\<close>
+	\<open>x2a = (x1b, x2b)\<close>
+	\<open>x2 = (x1a, x2a)\<close> and
+      conv: \<open>convert_state (virtual_copy (mset_set (extract_atms_clss CS {}))) T =
+       (x1, x2)\<close>
+     for uu ba S T Ta baa uua uub x1 x2 x1a x2a x1b x2b x1c x2c x1d x2d x1e x1f
+       x1g x2e x1h x2f x1i x2g x1j x2h x2i x2j x1k x2k
+  proof -
+      show \<open>x1i \<noteq> None\<close> 
+      using T conv nempty
+      unfolding st
+      by (cases x1i)
+       (auto simp: convert_state_def twl_st_heur_parsing_def
+         twl_st_heur_parsing_no_WL_def
+        isa_vmtf_init_def vmtf_init_def mset_set_empty_iff)
+    show \<open>x1j \<noteq> None\<close> 
+      using T conv nempty
+      unfolding st
+      by (cases x1i)
+       (auto simp: convert_state_def twl_st_heur_parsing_def
+         twl_st_heur_parsing_no_WL_def
+        isa_vmtf_init_def vmtf_init_def mset_set_empty_iff)
+  qed
+
+  have rewatch_heur_st_fast_pre: \<open>rewatch_heur_st_fast_pre
+	 (convert_state (virtual_copy (mset_set (extract_atms_clss CS {}))) T)\<close>
+    if 
+      T: \<open>(T, Ta)
+       \<in> twl_st_heur_parsing_no_WL (mset_set (extract_atms_clss CS {})) O
+	 {(S, T). S = remove_watched T \<and> get_watched_wl (fst T) = (\<lambda>_. [])}\<close> and
+      length_le: \<open>\<not>\<not>isasat_fast_init (convert_state (virtual_copy (mset_set (extract_atms_clss CS {}))) T)\<close>
+    for uu ba S T Ta baa uua uub
+  proof -
+    have \<open>valid_arena (get_clauses_wl_heur_init T) (get_clauses_wl (fst Ta))
+      (set (get_vdom_heur_init T))\<close>
+      using T by (auto simp: twl_st_heur_parsing_no_WL_def)
+    then show ?thesis
+      using length_le unfolding rewatch_heur_st_fast_pre_def convert_state_def
+        isasat_fast_init_def uint64_max_def uint32_max_def
+      by (auto dest: valid_arena_in_vdom_le_arena)
+  qed
+
+  have finalise_init_code2: \<open>finalise_init_code b Tb
+	\<le> SPEC (\<lambda>c. (c, finalise_init Tc) \<in>  {(S', T').
+             (S', T') \<in> twl_st_heur \<and>
+             get_clauses_wl_heur_init Tb = get_clauses_wl_heur S'})\<close>
+  if 
+    Ta: \<open>(T, Ta)
+     \<in> twl_st_heur_parsing_no_WL (mset_set (extract_atms_clss CS {})) O
+       {(S, T). S = remove_watched T \<and> get_watched_wl (fst T) = (\<lambda>_. [])}\<close> and
+    confl: \<open>\<not> get_conflict_wl (from_init_state Ta) \<noteq> None\<close> and
+    \<open>CS \<noteq> []\<close> and
+    nempty: \<open>extract_atms_clss CS {} \<noteq> {}\<close> and
+    \<open>isasat_input_bounded_nempty (mset_set (extract_atms_clss CS {}))\<close> and
+    clss_CS: \<open>mset `# ran_mf (get_clauses_wl (from_init_state Ta)) +
+     get_unit_clauses_wl (from_init_state Ta) =
+     mset `# mset CS\<close> and
+    learned: \<open>learned_clss_l (get_clauses_wl (from_init_state Ta)) = {#}\<close> and
+    \<open>virtual_copy (mset_set (extract_atms_clss CS {})) \<noteq> {#}\<close> and
+    \<open>isasat_input_bounded_nempty
+      (virtual_copy (mset_set (extract_atms_clss CS {})))\<close> and
+    \<open>case convert_state (virtual_copy (mset_set (extract_atms_clss CS {}))) T of
+     (M', N', D', Q', W', xa, xb) \<Rightarrow>
+       (case xa of
+        (x, xa) \<Rightarrow>
+          (case x of
+           (ns, m, fst_As, lst_As, next_search) \<Rightarrow>
+             \<lambda>to_remove (\<phi>, clvls). fst_As \<noteq> None \<and> lst_As \<noteq> None)
+           xa)
+        xb\<close> and
+    T: \<open>(Tb, Tc)
+     \<in> {(S, Ta'). (S, Ta')
+               \<in> twl_st_heur_parsing (mset_set (extract_atms_clss CS {})) \<and>
+               get_clauses_wl_heur_init S = get_clauses_wl_heur_init T \<and>
+               get_conflict_wl_heur_init S = get_conflict_wl_heur_init T \<and>
+              get_clauses_wl (fst Ta') = get_clauses_wl (fst Ta) \<and>
+               get_conflict_wl (fst Ta') = get_conflict_wl (fst Ta) \<and>
+               get_unit_clauses_wl (fst Ta') = get_unit_clauses_wl (fst Ta)} O
+       {(S, T). S = (T, {#})}\<close>
+    for uu ba S T Ta baa uua uub V W b Tb Tc
+  proof -
+    have 1: \<open>get_conflict_wl Tc = None\<close>
+      using confl T by (auto simp: from_init_state_def)
+    have 2: \<open>all_atms (get_clauses_wl Tc) (get_unit_clauses_wl Tc) \<noteq> {#}\<close>
+      using clss_CS[THEN arg_cong, of set_mset] clss_CS nempty T Ta
+      by (auto 5 5 simp flip: all_atms_def[symmetric] simp: all_lits_def
+        isasat_input_bounded_nempty_def extract_atms_clss_alt_def
+	all_lits_of_mm_empty_iff from_init_state_def)
+    have 3: \<open>set_mset (all_atms_st Tc) = set_mset (all_atms_st (fst Ta))\<close>
+      using T by auto
+    have 3: \<open>set_mset (all_atms_st Tc) = set_mset (mset_set (extract_atms_clss CS {}))\<close>
+      using clss_CS[THEN arg_cong, of set_mset, simplified] nempty T Ta
+      unfolding 3
+      by (auto simp flip: all_atms_def[symmetric] simp: all_lits_def
+        isasat_input_bounded_nempty_def from_init_state_def
+  	atm_of_all_lits_of_mm extract_atms_clss_alt_def atms_of_ms_def)
+
+    have H: \<open>A = B \<Longrightarrow> x \<in> A \<Longrightarrow> x \<in> B\<close> for A B x
+      by auto
+    have H': \<open>A = B \<Longrightarrow> A x \<Longrightarrow> B x\<close> for A B x
+      by auto
+
+    note cong =  trail_pol_cong
+      option_lookup_clause_rel_cong isa_vmtf_init_cong
+       vdom_m_cong[THEN H] isasat_input_nempty_cong[THEN iffD1]
+      isasat_input_bounded_cong[THEN iffD1]
+       cach_refinement_empty_cong[THEN H']
+       phase_saving_cong[THEN H']
+       \<L>\<^sub>a\<^sub>l\<^sub>l_cong[THEN H]
+       D\<^sub>0_cong[THEN H]
+
+    have 4: \<open>(convert_state (mset_set (extract_atms_clss CS {})) Tb, Tc)
+    \<in> twl_st_heur_post_parsing_wl\<close>
+      using T  nempty
+      by (auto simp: twl_st_heur_parsing_def twl_st_heur_post_parsing_wl_def
+        convert_state_def eq_commute[of \<open>mset _\<close> \<open>dom_m _\<close>]
+	vdom_m_cong[OF 3[symmetric]] \<L>\<^sub>a\<^sub>l\<^sub>l_cong[OF 3[symmetric]]
+	dest!: cong[OF 3[symmetric]])
+
+    show ?thesis
+      apply (rule finalise_init_finalise_init_full[unfolded conc_fun_RETURN,
+        THEN order_trans])
+      by (use 1 2 learned 4 T in \<open>auto simp: from_init_state_def convert_state_def\<close>)
+  qed
+  have isasat_fast: \<open>isasat_fast Td\<close>
+   if
+     fast: \<open>\<not> \<not> isasat_fast_init
+	   (convert_state (virtual_copy (mset_set (extract_atms_clss CS {})))
+	     T)\<close> and
+     Tb: \<open>(Tb, Tc)
+      \<in> {(S, Tb).
+	 (S, Tb) \<in> twl_st_heur_parsing (mset_set (extract_atms_clss CS {})) \<and>
+	 get_clauses_wl_heur_init S = get_clauses_wl_heur_init T \<and>
+	 get_conflict_wl_heur_init S = get_conflict_wl_heur_init T \<and>
+	 get_clauses_wl (fst Tb) = get_clauses_wl (fst Ta) \<and>
+	 get_conflict_wl (fst Tb) = get_conflict_wl (fst Ta) \<and>
+	 get_unit_clauses_wl (fst Tb) = get_unit_clauses_wl (fst Ta)} O
+	{(S, T). S = (T, {#})}\<close> and
+     Td: \<open>(Td, Te)
+      \<in> {(S', T').
+	 (S', T') \<in> twl_st_heur \<and>
+	 get_clauses_wl_heur_init Tb = get_clauses_wl_heur S'}\<close>
+    for uu ba S T Ta baa uua uub Tb Tc Td Te
+  proof -
+     show ?thesis
+       using fast Td Tb
+       by (auto simp: convert_state_def isasat_fast_init_def isasat_fast_def)
+  qed
   show ?thesis
     unfolding IsaSAT_heur_alt_def IsaSAT_alt_def
-    apply (refine_vcg virtual_copy init_state_wl_heur)
+    apply (refine_vcg virtual_copy init_state_wl_heur banner
+      cdcl_twl_stgy_restart_prog_wl_heur_cdcl_twl_stgy_restart_prog_wl_D[THEN fref_to_Down])
     subgoal by (rule input_le)
     subgoal by (rule distinct_mset_mset_set)
     subgoal by auto
@@ -1858,35 +2260,86 @@ proof -
        init_state_wl_def init_state_wl_heur_def
        inres_def RES_RES_RETURN_RES
        RES_RETURN_RES)
-       
-    subgoal
-    using rewatch_heur_rewatch
-       oops
-find_theorems valid_arena fmempty
+    apply (rule rewatch_heur_st_rewatch_st; assumption)
+    subgoal unfolding convert_state_def by (rule get_conflict_wl_is_None_heur_init)
+    subgoal by (simp add: empty_init_code_def)
+    subgoal by simp
+    subgoal by (simp add: empty_conflict_code_def op_arl_empty_def)
+    subgoal by (simp add: mset_set_empty_iff extract_atms_clss_alt_def)
+    subgoal by simp
+    subgoal by (rule finalise_init_nempty)
+    subgoal by (rule finalise_init_nempty)
+    apply (rule finalise_init_code; assumption)
+    subgoal by fast
+    subgoal by fast
+    subgoal premises p for _ ba S T Ta Tb Tc u v
+      using p(28)
+      by (auto simp: twl_st_heur_def get_conflict_wl_is_None_heur_def
+        extract_stats_def extract_state_stat_def
+	option_lookup_clause_rel_def trail_pol_def
+	extract_model_of_state_def rev_map
+	extract_model_of_state_stat_def
+	dest!: ann_lits_split_reasons_map_lit_of)
 
-    thm init_dt_wl_heur_init_dt_wl[THEN fref_to_Down_curry,
-      of \<open>mset_set (extract_atms_clss CS {})\<close>]
-    thm rewatch_heur_rewatch
+    apply (rule init_dt_wl_heur[of \<open>mset_set (extract_atms_clss CS {})\<close>])
+    subgoal by (auto simp: lits_C)
+    subgoal by (auto simp: twl_st_heur_parsing_no_WL_wl_def
+       twl_st_heur_parsing_no_WL_def to_init_state_def
+       init_state_wl_def init_state_wl_heur_def
+       inres_def RES_RES_RETURN_RES
+       RES_RETURN_RES)
+    subgoal for _ S T U V by (rule get_conflict_wl_is_None_heur_init2)
+    subgoal by (simp add: empty_init_code_def)
+    subgoal by simp
+    subgoal by (simp add: empty_conflict_code_def op_arl_empty_def)
+    subgoal by simp
+    subgoal by simp
+    subgoal by (simp add: mset_set_empty_iff extract_atms_clss_alt_def)
+    subgoal by simp
+    subgoal by (rule finalise_init2)
+    subgoal by (rule finalise_init2)
+    apply (subst rewatch_heur_st_fast_def[symmetric])
+    apply (rule rewatch_heur_st_rewatch_st2; assumption)
+    apply (rule finalise_init_code2; assumption)
+    subgoal by fast
+    subgoal by fast
 
-    find_theorems init_dt_wl_heur init_dt_wl
-    find_theorems  rewatch_heur rewatch
-    thm init_dt_wl_heur_init_dt_wl
-    thm rewatch_heur_rewatch
-    term init_dt_wl'
+    subgoal premises p for _ ba S T Ta Tb Tc u v
+      using p(31)
+      by (auto simp: twl_st_heur_def get_conflict_wl_is_None_heur_def
+        extract_stats_def extract_state_stat_def
+	option_lookup_clause_rel_def trail_pol_def
+	extract_model_of_state_def rev_map
+	extract_model_of_state_stat_def
+	dest!: ann_lits_split_reasons_map_lit_of)
+    subgoal by (simp add: mset_set_empty_iff extract_atms_clss_alt_def)
+    subgoal by simp
+    subgoal by (rule finalise_init2)
+    subgoal by (rule finalise_init2)
+    subgoal for uu ba S T Ta baa uua uub
+      by (rule rewatch_heur_st_fast_pre)
+    apply (rule rewatch_heur_st_rewatch_st2; assumption)
+    apply (rule finalise_init_code2; assumption)
+    subgoal for uu ba S T Ta baa uua uub Tb Tc Td Te
+      by (rule isasat_fast)
+    apply (rule cdcl_twl_stgy_restart_prog_early_wl_heur_cdcl_twl_stgy_restart_prog_early_wl_D[
+      THEN fref_to_Down])
+    subgoal by fast
+    subgoal by fast
+    subgoal premises p for _ ba S T Ta Tb Tc u v
+      using p(33)
+      by (auto simp: twl_st_heur_def get_conflict_wl_is_None_heur_def
+        extract_stats_def extract_state_stat_def
+	option_lookup_clause_rel_def trail_pol_def
+	extract_model_of_state_def rev_map
+	extract_model_of_state_stat_def
+	dest!: ann_lits_split_reasons_map_lit_of)
+    done
+qed
 
-
-
-lemma in_class_in_literals_are_in_\<L>\<^sub>i\<^sub>n:
-  assumes \<open>C \<in> set CS\<close>
-  shows \<open>literals_are_in_\<L>\<^sub>i\<^sub>n (mset_set (extract_atms_clss CS {})) (mset C)\<close>
-  apply (auto simp: literals_are_in_\<L>\<^sub>i\<^sub>n_def extract_atms_clss_alt_def
-      \<L>\<^sub>a\<^sub>l\<^sub>l_def all_lits_of_m_def)
-  apply (subst insert_absorb[OF assms, symmetric])
-  apply auto
-  apply (subst (asm)insert_absorb[OF assms, symmetric])
-  apply (subst insert_absorb[OF assms, symmetric])
-  apply auto
-  done
+lemma isasat_fast_init_alt_def:
+  \<open>RETURN o isasat_fast_init = (\<lambda>(M, N, _). RETURN (length N \<le> 18446744069414584315))\<close>
+  by (auto simp: isasat_fast_init_def uint64_max_def uint32_max_def intro!: ext)
 
 (*
 lemma cdcl_twl_stgy_prog_wl_D_break_fast_code_ref':
@@ -2058,12 +2511,13 @@ lemma length_get_clauses_wl_heur_init_alt_def:
   unfolding length_get_clauses_wl_heur_init_def
   by auto
 
-sepref_definition length_get_clauses_wl_heur_init_code
-  is \<open>RETURN o length_get_clauses_wl_heur_init\<close>
-  :: \<open>isasat_init_assn\<^sup>k \<rightarrow>\<^sub>a nat_assn\<close>
-  unfolding length_get_clauses_wl_heur_init_alt_def isasat_init_assn_def
+sepref_definition isasat_fast_init_code
+  is \<open>RETURN o isasat_fast_init\<close>
+  :: \<open>isasat_init_assn\<^sup>k \<rightarrow>\<^sub>a bool_assn\<close>
+  unfolding isasat_fast_init_alt_def isasat_init_assn_def
   by sepref
-declare length_get_clauses_wl_heur_init_code.refine[sepref_fr_rules]
+  
+declare isasat_fast_init_code.refine[sepref_fr_rules]
 
 declare convert_state_hnr[sepref_fr_rules]
   convert_state_hnr_unb[sepref_fr_rules]
@@ -2191,754 +2645,6 @@ export_code IsaSAT_code
     uint32_of_nat
   in SML_imp module_name SAT_Solver file "code/IsaSAT_solver.sml"
 
-definition TWL_to_clauses_state_conv :: \<open>(nat twl_st_wl \<times> nat cdcl\<^sub>W_restart_mset) set\<close> where
-  \<open>TWL_to_clauses_state_conv = twl_st_of_wl None O {(S', S). S = state\<^sub>W_of S'}\<close>
-
-lemma extract_atms_cls_empty_iff: \<open>extract_atms_cls Cs C0 = {} \<longleftrightarrow> (C0 = {} \<and> Cs = [])\<close>
-  unfolding extract_atms_cls_def
-  by (induction Cs arbitrary: C0) force+
-
-lemma extract_atms_clss_empty_iff:
-   \<open>extract_atms_clss CS C0  = {} \<longleftrightarrow> (C0 = {} \<and> (\<forall>C \<in> set CS. C = []))\<close>
-  unfolding extract_atms_clss_alt_def
-  by auto
-
-lemma is_\<L>\<^sub>a\<^sub>l\<^sub>l_extract_atms_clss:
-    \<open>is_\<L>\<^sub>a\<^sub>l\<^sub>l (mset_set (extract_atms_clss CS' {}))
-       (all_lits_of_mm (mset `# mset CS'))\<close>
-proof -
-  have [simp]: \<open>is_neg xb \<Longrightarrow> Pos (atm_of xb) = - xb\<close> for xb
-    by (cases xb) auto
-  have [simp]: \<open>is_pos xb \<Longrightarrow> Neg (atm_of xb) = - xb\<close> for xb
-    by (cases xb) auto
-  have [intro]: \<open>\<And>x. x \<in># all_lits_of_mm
-               (mset `# mset CS') \<Longrightarrow>
-         x \<notin> Neg `
-              (\<Union>C\<in>set CS'. atm_of ` set C) \<Longrightarrow>
-         x \<in> Pos ` (\<Union>C\<in>set CS'. atm_of ` set C)\<close>
-    apply (induction CS')
-    subgoal by auto
-    subgoal for C CS x
-      by (cases x)
-        (auto simp: all_lits_of_mm_add_mset image_Un in_all_lits_of_m_ain_atms_of_iff
-        atm_of_eq_atm_of uminus_lit_swap)
-    done
-  show ?thesis
-    by (auto simp: extract_atms_clss_alt_def
-          is_\<L>\<^sub>a\<^sub>l\<^sub>l_def \<L>\<^sub>a\<^sub>l\<^sub>l_def all_lits_of_mm_add_mset
-          all_lits_of_m_add_mset
-        dest!: split_list)
-qed
-
-(* TODO Move *)
-
-lemma finite_extract_atms_clss[simp]: \<open>finite (extract_atms_clss CS' {})\<close> for CS'
-  by (auto simp: extract_atms_clss_alt_def)
-
-lemma in_\<L>\<^sub>a\<^sub>l\<^sub>l_extract_atms_clss_in_all_lits_of_mm:
-  shows \<open>L \<in># \<L>\<^sub>a\<^sub>l\<^sub>l (mset_set (extract_atms_clss CS' {})) \<longleftrightarrow>
-    L \<in># all_lits_of_mm (mset `# mset CS')\<close>
-    (is \<open>?A \<longleftrightarrow> ?B\<close>)
-proof -
-  have 1: \<open>?A \<longleftrightarrow> L \<in># all_lits_of_m (mset_set (Pos ` extract_atms_clss CS' {}))\<close>
-    unfolding \<L>\<^sub>a\<^sub>l\<^sub>l_def
-    by (cases L)
-       (auto simp: in_all_lits_of_m_ain_atms_of_iff atms_of_def image_image)
-  also have \<open>\<dots> \<longleftrightarrow> ?B\<close>
-    using 1 is_\<L>\<^sub>a\<^sub>l\<^sub>l_extract_atms_clss is_\<L>\<^sub>a\<^sub>l\<^sub>l_def by auto
-  finally show ?thesis .
-qed
-
-lemma [simp]: \<open>is_\<L>\<^sub>a\<^sub>l\<^sub>l (all_atms N NE) (all_lits N NE)\<close>
-proof -
-  define NUE where \<open>NUE \<equiv> {#mset (fst C). C \<in># ran_m N#} + NE\<close>
-  show ?thesis
-  unfolding is_\<L>\<^sub>a\<^sub>l\<^sub>l_def all_atms_def all_lits_def \<L>\<^sub>a\<^sub>l\<^sub>l_def NUE_def[symmetric]
-  apply (auto simp: in_all_lits_of_mm_ain_atms_of_iff atm_of_all_lits_of_mm
-    image_image[symmetric])
-  by (metis (full_types) Neg_atm_of_iff Pos_atm_of_iff imageI)
-qed
-
-lemma cdcl\<^sub>W_cdcl\<^sub>W_init_state:
-  \<open>cdcl\<^sub>W_restart_mset.cdcl\<^sub>W (init_state {#}) S \<longleftrightarrow> False\<close>
-  using cdcl\<^sub>W_ex_cdcl\<^sub>W_stgy cdcl\<^sub>W_stgy_cdcl\<^sub>W_init_state_empty_no_step by blast
-
-lemma rtranclp_cdcl\<^sub>W_init_state:
-  \<open>cdcl\<^sub>W_restart_mset.cdcl\<^sub>W_stgy\<^sup>*\<^sup>* (M, CS, {#}, Some {#}) S \<longleftrightarrow> S = (M, CS, {#}, Some {#})\<close>
-  unfolding full_def rtranclp_unfold
-  by (subst tranclp_unfold_begin)
-     (auto simp:  cdcl\<^sub>W_restart_mset.cdcl\<^sub>W_stgy.simps
-      cdcl\<^sub>W_restart_mset.conflict.simps cdcl\<^sub>W_restart_mset.cdcl\<^sub>W_o.simps
-       cdcl\<^sub>W_restart_mset.propagate.simps cdcl\<^sub>W_restart_mset.decide.simps
-       cdcl\<^sub>W_restart_mset.cdcl\<^sub>W_bj.simps cdcl\<^sub>W_restart_mset.backtrack.simps
-      cdcl\<^sub>W_restart_mset.skip.simps cdcl\<^sub>W_restart_mset.resolve.simps
-      cdcl\<^sub>W_restart_mset_state clauses_def)
-
-lemma (in -) added_only_watched[simp]:
-  assumes \<open>(T, T') \<in> added_only_watched \<close>
-  shows
-     \<open>get_conflict_init_wl T' = get_conflict_wl (fst T)\<close>
-     \<open>get_trail_init_wl T' = get_trail_wl (fst T)\<close>
-  using assms by (auto simp: added_only_watched_def)
-
-lemma cdcl_twl_stgy_prog_wl_spec_final2:
-  shows
-    \<open>(SAT_wl, SAT) \<in> [\<lambda>CS. (\<forall>C \<in># CS. distinct_mset C) \<and>
-        (\<forall>C \<in># CS. \<forall>L \<in># C. nat_of_lit L \<le> uint_max)]\<^sub>f
-     (list_mset_rel O \<langle>list_mset_rel\<rangle> mset_rel) \<rightarrow> \<langle>TWL_to_clauses_state_conv\<rangle>nres_rel\<close>
-proof -
-  have in_list_mset_rel: \<open>(CS', y) \<in> list_mset_rel \<longleftrightarrow> y = mset CS'\<close> for CS' y
-    by (auto simp: list_mset_rel_def br_def)
-  have in_list_mset_rel_mset_rel:
-    \<open>(mset CS', CS) \<in> \<langle>list_mset_rel\<rangle>mset_rel \<longleftrightarrow> CS = mset `# mset CS'\<close> for CS CS'
-    by (auto simp: list_mset_rel_def br_def mset_rel_def p2rel_def rel_mset_def
-        rel2p_def[abs_def] list_all2_op_eq_map_right_iff')
-
-  have \<L>\<^sub>a\<^sub>l\<^sub>l:
-    \<open>is_\<L>\<^sub>a\<^sub>l\<^sub>l (mset_set (extract_atms_clss CS' {})) (all_lits_of_mm (mset `# mset CS'))\<close>
-    for CS'
-    by (auto simp add: is_\<L>\<^sub>a\<^sub>l\<^sub>l_extract_atms_clss)
-  have extract_nempty: \<open>extract_atms_clss xs {} = {} \<longleftrightarrow> set xs = {[]}\<close>
-  if
-    H: \<open>Multiset.Ball ys distinct_mset \<and> (\<forall>C\<in>#ys. \<forall>L\<in>#C. nat_of_lit L \<le> uint_max)\<close> and
-    rel: \<open>(xs, ys) \<in> list_mset_rel O \<langle>list_mset_rel\<rangle>mset_rel\<close> and
-    le_xs: \<open>length xs \<noteq> 0\<close>
-    for xs ys
-    using le_xs unfolding extract_atms_clss_alt_def by (cases xs) auto
-
-  have [simp]: \<open>isasat_input_bounded (mset_set (extract_atms_clss CS' {}))\<close>
-    if CS_p: \<open>\<forall>C\<in>set CS'. \<forall>L\<in>set C. nat_of_lit L \<le> uint_max\<close>
-    for CS'
-    unfolding isasat_input_bounded_def
-  proof
-    fix L
-    assume L: \<open>L \<in># \<L>\<^sub>a\<^sub>l\<^sub>l (mset_set (extract_atms_clss CS' {}))\<close>
-    then obtain C where
-      L: \<open>C\<in>set CS' \<and> (L \<in>set C \<or> - L \<in> set C)\<close>
-      apply (cases L)
-      apply (auto simp: extract_atms_clss_alt_def uint_max_def nat_of_uint32_uint32_of_nat_id
-          \<L>\<^sub>a\<^sub>l\<^sub>l_def)+
-      apply (metis literal.exhaust_sel)+
-      done
-    have \<open>nat_of_lit L \<le> uint_max \<or> nat_of_lit (-L) \<le> uint_max\<close>
-      using L CS_p by auto
-    then show \<open>nat_of_lit L \<le> uint_max\<close>
-      using L
-      by (cases L) (auto simp: extract_atms_clss_alt_def uint_max_def)
-  qed
-
-  have conflict_during_init: \<open>RETURN (fst T)
-      \<le> \<Down> TWL_to_clauses_state_conv
-           (SPEC (conclusive_CDCL_run CS (init_state CS)))\<close>
-    if
-      \<open>Multiset.Ball CS distinct_mset \<and> (\<forall>C\<in>#CS. \<forall>L\<in>#C. nat_of_lit L \<le> uint_max)\<close> and
-      CS'_CS: \<open>(CS', CS) \<in> list_mset_rel O \<langle>list_mset_rel\<rangle>mset_rel\<close> and
-      spec: \<open>init_dt_wl_spec_full CS' (([], fmempty, None, {#}, {#}, {#}), {#}) T\<close> and
-      confl: \<open>get_conflict_wl (fst T) \<noteq> None\<close>
-    for T CS CS'
-  proof -
-    obtain U V T' W where
-      U: \<open>((([], fmempty, None, {#}, {#}, {#}), {#}), U) \<in> state_wl_l_init\<close> and
-      T_V: \<open>(T', V) \<in> state_wl_l_init\<close> and
-      \<open>correct_watching_init (fst T)\<close> and
-      T_T': \<open>(T, T') \<in> added_only_watched\<close> and
-      V_W: \<open>(V, W) \<in> twl_st_l_init\<close> and
-      struct_invs: \<open>twl_struct_invs_init W\<close> and
-      \<open>clauses_to_update_l_init V = {#}\<close> and
-      count_dec: \<open>\<forall>s\<in>set (get_trail_l_init V). \<not> is_decided s\<close> and
-      \<open>get_conflict_l_init V = None \<longrightarrow>
-         literals_to_update_l_init V =
-         uminus `# lit_of `# mset (get_trail_l_init V)\<close> and
-      clss: \<open>mset `# mset CS' + mset `# ran_mf (get_clauses_l_init U) +
-        other_clauses_l_init U +  get_unit_clauses_l_init U =
-        mset `# ran_mf (get_clauses_l_init V) + other_clauses_l_init V +
-          get_unit_clauses_l_init V\<close> and
-      learned_UV: \<open>learned_clss_lf (get_clauses_l_init U) =
-        learned_clss_lf (get_clauses_l_init V)\<close> and
-      learned: \<open>get_learned_unit_clauses_l_init V = get_learned_unit_clauses_l_init U\<close> and
-      \<open>twl_list_invs (fst V)\<close> and
-      \<open>twl_stgy_invs (fst W)\<close> and
-      \<open>other_clauses_l_init V \<noteq> {#} \<longrightarrow> get_conflict_l_init V \<noteq> None\<close> and
-      \<open>{#} \<in># mset `# mset CS' \<longrightarrow> get_conflict_l_init V \<noteq> None\<close> and
-      \<open>get_conflict_l_init U \<noteq> None \<longrightarrow>
-      get_conflict_l_init U = get_conflict_l_init V\<close>
-      using spec unfolding init_dt_wl_spec_def init_dt_spec_def
-        init_dt_wl_spec_full_def apply -
-      apply normalize_goal+
-      apply (rename_tac U T' V W)
-      by presburger
-
-    have learned_U: \<open>learned_clss_lf (get_clauses_l_init U) = {#}\<close>
-          \<open>get_clauses_l_init U = fmempty\<close>
-          \<open>other_clauses_l_init U  = {#}\<close>
-          \<open>get_unit_clauses_l_init U = {#}\<close>
-      using U T_V V_W T_T'
-      by (cases U; auto simp: state_wl_l_init_def state_wl_l_def
-         added_only_watched_def state_wl_l_init'_def; fail)+
-    then have learned_W: \<open>get_learned_clauses_init W = {#}\<close> \<open>get_unit_learned_clauses_init W = {#}\<close>
-      \<open>get_unit_init_clauses_init W = get_unit_clauses_l_init V\<close>
-      using U T_V V_W learned learned_UV by (cases T; cases U; cases V;
-         auto simp: state_wl_l_init_def state_wl_l_def twl_st_l_init_def; fail)+
-    have ran_m_init_U:
-      \<open>ran_m (get_clauses_l_init V) = init_clss_l (get_clauses_l_init V)\<close>
-      using U T_V V_W learned learned_UV learned_U
-      apply (subst all_clss_l_ran_m[symmetric])
-      by (cases T; cases U; cases V;
-         auto simp: state_wl_l_init_def state_wl_l_def twl_st_l_init_def
-         simp del: all_clss_l_ran_m)
-    have [simp]: \<open>get_trail_init_wl T' = get_trail_wl (fst T)\<close>
-      \<open>other_clauses_init_wl T' = snd T\<close>
-      \<open>get_conflict_init_wl T' = get_conflict_wl (fst T)\<close>
-      using T_T' by (auto simp: added_only_watched_def)
-    have
-      \<open>clause `# (get_init_clauses_init W) =
-       mset `# (init_clss_lf (get_clauses_l_init V))\<close>
-      using U T_V V_W learned learned_UV by (cases T; cases U; cases V;
-         auto simp: state_wl_l_init_def state_wl_l_def twl_st_l_init_def
-         mset_take_mset_drop_mset' mset_take_mset_drop_mset
-         dest!: multi_member_split)
-    from arg_cong[OF this, of set_mset]
-    have init_clss_W_V: \<open>clause ` set_mset (get_init_clauses_init W)
-        = mset ` set_mset (init_clss_lf (get_clauses_l_init V))\<close>
-      by auto
-    have count_dec: \<open>count_decided (get_trail_wl (fst T)) = 0\<close>
-      using count_dec T_V V_W unfolding count_decided_0_iff by (auto simp: twl_st_init
-          twl_st_wl_init)
-    have CS: \<open>CS = mset `# mset CS'\<close>
-      using CS'_CS by (auto simp: in_list_mset_rel in_list_mset_rel_mset_rel)
-
-    have le: \<open>cdcl\<^sub>W_restart_mset.cdcl\<^sub>W_learned_clause (state\<^sub>W_of_init W)\<close> and
-      all_struct_invs:
-        \<open>cdcl\<^sub>W_restart_mset.cdcl\<^sub>W_all_struct_inv (state\<^sub>W_of_init W)\<close>
-      using struct_invs unfolding twl_struct_invs_init_def
-         cdcl\<^sub>W_restart_mset.cdcl\<^sub>W_all_struct_inv_def
-      by fast+
-    have \<open>cdcl\<^sub>W_restart_mset.cdcl\<^sub>W_conflicting (state\<^sub>W_of_init W)\<close>
-      using struct_invs unfolding twl_struct_invs_init_def
-        cdcl\<^sub>W_restart_mset.cdcl\<^sub>W_all_struct_inv_def
-      by fast
-    have \<open>unsatisfiable (set_mset (mset `# mset (rev CS')))\<close>
-      using conflict_of_level_unsatisfiable[OF all_struct_invs] count_dec confl learned clss T_V V_W
-        learned_U init_clss_W_V learned_W le ran_m_init_U
-      by (auto simp: clauses_def mset_take_mset_drop_mset' twl_st_init twl_st_wl_init image_image
-          cdcl\<^sub>W_restart_mset.cdcl\<^sub>W_learned_clauses_entailed_by_init_def ac_simps twl_st_l_init)
-    then have unsat[simp]: \<open>unsatisfiable (mset ` set CS')\<close>
-      by auto
-    then have [simp]: \<open>CS' \<noteq> []\<close>
-      by (auto simp del: unsat)
-    have T_V': \<open>(fst T, fst V) \<in> state_wl_l None\<close>
-      using T_V T_T' by (cases V) (auto simp:state_wl_l_init_def added_only_watched_def
-        state_wl_l_def state_wl_l_init'_def)
-    show ?thesis
-      unfolding conclusive_CDCL_run_def
-      apply (rule RETURN_SPEC_refine)
-      apply (rule exI[of _ \<open>state\<^sub>W_of (fst W)\<close>])
-      apply (intro conjI)
-      subgoal
-        using T_V' V_W unfolding state_wl_l_init_def twl_st_l_init_alt_def
-        by (auto simp: TWL_to_clauses_state_conv_def mset_take_mset_drop_mset'
-            clauses_def in_list_mset_rel in_list_mset_rel_mset_rel)
-      subgoal
-        apply (rule disjI2)
-        using \<L>\<^sub>a\<^sub>l\<^sub>l struct_invs learned count_dec U clss confl T_V V_W
-        by (clarsimp simp: CS twl_st_init twl_st_wl_init twl_st_l_init)
-      done
-  qed
-
-  have empty_clss:
-   \<open>RETURN ([], fmempty, None, {#}, {#}, {#}, \<lambda>_. undefined)
-      \<le> \<Down> TWL_to_clauses_state_conv
-          (SPEC (conclusive_CDCL_run CS (init_state CS)))\<close>
-    if
-      \<open>Multiset.Ball CS distinct_mset \<and> (\<forall>C\<in>#CS. \<forall>L\<in>#C. nat_of_lit L \<le> uint_max)\<close> and
-      CS'_CS: \<open>(CS', CS) \<in> list_mset_rel O \<langle>list_mset_rel\<rangle>mset_rel\<close> and
-      spec: \<open>init_dt_wl_spec_full CS' (([], fmempty, None, {#}, {#}, {#}), {#}) T\<close> and
-      confl: \<open>\<not> get_conflict_wl (fst T) \<noteq> None\<close> and
-      [simp]: \<open>CS' = []\<close>
-    for CS' CS T
-  proof -
-    let ?init = \<open>([], {#}, {#}, None) :: nat cdcl\<^sub>W_restart_mset\<close>
-    let ?init_twl = \<open>([], {#}, {#}, None, {#}, {#}, {#}, {#}) :: nat twl_st\<close>
-    let ?init_l = \<open>([], fmempty, None, {#}, {#}, {#}, {#}) :: nat twl_st_l\<close>
-    let ?init_wl = \<open>([], fmempty, None, {#}, {#}, {#}, \<lambda>_. undefined) :: nat twl_st_wl\<close>
-    have [simp]: \<open>CS = {#}\<close>
-      using CS'_CS by (auto simp: in_list_mset_rel in_list_mset_rel_mset_rel)
-    have [simp]: \<open>full cdcl\<^sub>W_restart_mset.cdcl\<^sub>W_stgy ?init ?init\<close>
-      using full_cdcl\<^sub>W_init_state[of \<open>([], {#}, {#}, None)\<close>] by auto
-    have eq: \<open>twl_st_of_wl None = state_wl_l None O twl_st_l None\<close>
-      by (auto intro!: ext)
-    have \<open>(?init_twl, ?init) \<in> {(S', S). S = state\<^sub>W_of S'}\<close>
-      by auto
-    moreover have \<open>(?init_l, ?init_twl) \<in> twl_st_l None\<close>
-      by (auto simp: twl_st_l_def)
-    moreover have \<open>(?init_wl, ?init_l) \<in> state_wl_l None\<close>
-      by (auto simp: state_wl_l_def)
-    ultimately have \<open>(?init_wl, ?init)
-       \<in> (state_wl_l None O twl_st_l None) O {(S', S). S = state\<^sub>W_of S'}\<close>
-      by fast
-
-    then show ?thesis
-      using spec confl
-      unfolding init_dt_wl_spec_def conclusive_CDCL_run_def apply -
-      apply (rule RETURN_SPEC_refine)
-      apply (rule exI[of _ \<open>([], {#}, {#}, None)\<close>])
-      apply (intro conjI)
-      subgoal
-        unfolding TWL_to_clauses_state_conv_def eq
-        by assumption
-      subgoal
-        by (auto simp: cdcl\<^sub>W_cdcl\<^sub>W_init_state[unfolded init_state.simps])
-      done
-  qed
-
-  have extract_atms_clss_not_nil: \<open>extract_atms_clss CS' {} \<noteq> {}\<close>
-    if
-      \<open>Multiset.Ball CS distinct_mset \<and> (\<forall>C\<in>#CS. \<forall>L\<in>#C. nat_of_lit L \<le> uint_max)\<close> and
-      CS'_CS: \<open>(CS', CS) \<in> list_mset_rel O \<langle>list_mset_rel\<rangle>mset_rel\<close> and
-      spec: \<open>init_dt_wl_spec_full CS' (([], fmempty, None, {#}, {#}, {#}), {#}) T\<close> and
-      confl: \<open>\<not> get_conflict_wl (fst T) \<noteq> None\<close> and
-      [simp]: \<open>CS' \<noteq> []\<close>
-    for CS' CS T
-  proof -
-    obtain U V T' W where
-      U: \<open>((([], fmempty, None, {#}, {#}, {#}), {#}), U) \<in> state_wl_l_init\<close> and
-      T_V: \<open>(T', V) \<in> state_wl_l_init\<close> and
-      \<open>correct_watching_init (fst T)\<close> and
-      T_T': \<open>(T, T') \<in> added_only_watched\<close> and
-      V_W: \<open>(V, W) \<in> twl_st_l_init\<close> and
-      struct_invs: \<open>twl_struct_invs_init W\<close> and
-      \<open>clauses_to_update_l_init V = {#}\<close> and
-      count_dec: \<open>\<forall>s\<in>set (get_trail_l_init V). \<not> is_decided s\<close> and
-      \<open>get_conflict_l_init V = None \<longrightarrow>
-         literals_to_update_l_init V =
-         uminus `# lit_of `# mset (get_trail_l_init V)\<close> and
-      clss: \<open>mset `# mset CS' + mset `# ran_mf (get_clauses_l_init U) +
-        other_clauses_l_init U +  get_unit_clauses_l_init U =
-        mset `# ran_mf (get_clauses_l_init V) + other_clauses_l_init V +
-          get_unit_clauses_l_init V\<close> and
-      learned_UV: \<open>learned_clss_lf (get_clauses_l_init U) =
-        learned_clss_lf (get_clauses_l_init V)\<close> and
-      learned: \<open>get_learned_unit_clauses_l_init V = get_learned_unit_clauses_l_init U\<close> and
-      \<open>twl_list_invs (fst V)\<close> and
-      \<open>twl_stgy_invs (fst W)\<close> and
-      snd_T_conflict: \<open>other_clauses_l_init V \<noteq> {#} \<longrightarrow> get_conflict_l_init V \<noteq> None\<close> and
-      false_in_conflict: \<open>{#} \<in># mset `# mset CS' \<longrightarrow> get_conflict_l_init V \<noteq> None\<close> and
-      \<open>get_conflict_l_init U \<noteq> None \<longrightarrow>
-        get_conflict_l_init U = get_conflict_l_init V\<close>
-      using spec unfolding init_dt_wl_spec_def init_dt_spec_def
-        init_dt_wl_spec_full_def apply -
-      apply normalize_goal+
-      apply (rename_tac U T' V W)
-      by presburger
-    have CS: \<open>CS = mset `# mset CS'\<close>
-      using CS'_CS by (auto simp: in_list_mset_rel in_list_mset_rel_mset_rel)
-    have \<open>other_clauses_init_wl T' = {#}\<close>
-      using snd_T_conflict confl T_V V_W T_T' by (auto simp: added_only_watched_def
-         state_wl_l_init_def state_wl_l_init'_def twl_st_l_init_def)
-    have \<open>\<exists>C\<in>set CS'. C \<noteq> []\<close>
-    proof (rule ccontr)
-      assume \<open>\<not> ?thesis\<close>
-      then have E: \<open>\<forall>C\<in>set CS'. C = []\<close>
-        by blast
-      show False
-        by (cases CS'; cases T; cases T')
-          (use E false_in_conflict clss confl T_V V_W T_T' in
-            \<open>auto simp: clauses_def CS state_wl_l_init_def state_wl_l_init'_def twl_st_l_init_def
-            added_only_watched_def\<close>)
-    qed
-    then show ?thesis
-      unfolding extract_atms_clss_empty_iff by auto
-  qed
-
-  have CDCL_steps:
-    \<open>cdcl_twl_stgy_restart_prog_wl_D (fst T)
-      \<le> \<Down> TWL_to_clauses_state_conv
-          (SPEC (conclusive_CDCL_run CS (init_state CS)))\<close>
-      (is ?steps is \<open>_ \<le> \<Down> _ ?Spec\<close>) and
-    clauses: \<open>mset `# ran_mf (get_clauses_wl (fst T)) +
-         get_unit_clauses_wl (fst T) = mset `# mset CS'\<close>
-        (is ?clss) and
-    break_CDCL_steps: \<open>cdcl_twl_stgy_restart_prog_wl_D (fst T)
-    \<le> \<Down> TWL_to_clauses_state_conv (SPEC (conclusive_CDCL_run CS (init_state CS)))\<close>
-      (is ?break_steps) and
-    learned_clss: \<open>learned_clss_l (get_clauses_wl (fst T)) = {#}\<close> (is ?learned_clss)
-    if
-      CS_p: \<open>Multiset.Ball CS distinct_mset \<and> (\<forall>C\<in>#CS. \<forall>L\<in>#C. nat_of_lit L \<le> uint_max)\<close> and
-      CS'_CS: \<open>(CS', CS) \<in> list_mset_rel O \<langle>list_mset_rel\<rangle>mset_rel\<close> and
-      spec: \<open>init_dt_wl_spec_full CS' (([], fmempty, None, {#}, {#}, {#}), {#}) T\<close> and
-      confl: \<open>\<not> get_conflict_wl (fst T) \<noteq> None\<close> and
-      CS'_nempty: \<open>CS' \<noteq> []\<close> and
-      \<open>extract_atms_clss CS' {} \<noteq> {}\<close> and
-      [simp]: \<open>isasat_input_bounded_nempty (mset_set (extract_atms_clss CS' {}))\<close>
-    for CS' CS T
-  proof -
-    obtain U V T' W where
-      U: \<open>((([], fmempty, None, {#}, {#}, {#}), {#}), U) \<in> state_wl_l_init\<close> and
-      T_V: \<open>(T', V) \<in> state_wl_l_init\<close> and
-      corr_w: \<open>correct_watching_init (fst T)\<close> and
-      T_T': \<open>(T, T') \<in> added_only_watched\<close> and
-      V_W: \<open>(V, W) \<in> twl_st_l_init\<close> and
-      struct_invs: \<open>twl_struct_invs_init W\<close> and
-      clss_upd: \<open>clauses_to_update_l_init V = {#}\<close> and
-      count_dec: \<open>\<forall>s\<in>set (get_trail_l_init V). \<not> is_decided s\<close> and
-      \<open>get_conflict_l_init V = None \<longrightarrow>
-         literals_to_update_l_init V =
-         uminus `# lit_of `# mset (get_trail_l_init V)\<close> and
-      clss: \<open>mset `# mset CS' + mset `# ran_mf (get_clauses_l_init U) +
-        other_clauses_l_init U +  get_unit_clauses_l_init U =
-        mset `# ran_mf (get_clauses_l_init V) + other_clauses_l_init V +
-          get_unit_clauses_l_init V\<close> and
-      learned_UV: \<open>learned_clss_lf (get_clauses_l_init U) =
-        learned_clss_lf (get_clauses_l_init V)\<close> and
-      learned: \<open>get_learned_unit_clauses_l_init V = get_learned_unit_clauses_l_init U\<close> and
-      add_invs: \<open>twl_list_invs (fst V)\<close> and
-      stgy_invs: \<open>twl_stgy_invs (fst W)\<close> and
-      snd_T_conflict: \<open>other_clauses_l_init V \<noteq> {#} \<longrightarrow> get_conflict_l_init V \<noteq> None\<close> and
-      false_in_conflict: \<open>{#} \<in># mset `# mset CS' \<longrightarrow> get_conflict_l_init V \<noteq> None\<close> and
-      \<open>get_conflict_l_init U \<noteq> None \<longrightarrow>
-        get_conflict_l_init U = get_conflict_l_init V\<close>
-      using spec unfolding init_dt_wl_spec_def init_dt_spec_def
-        init_dt_wl_spec_full_def apply -
-      apply normalize_goal+
-      apply (rename_tac U T' V W)
-      by presburger
-    have snd_T: \<open>other_clauses_init_wl T' = {#}\<close>
-      using confl snd_T_conflict T_V V_W T_T'
-      by (auto simp: twl_st_init twl_st_l_init twl_st_wl_init)
-    have
-      struct_invs: \<open>twl_struct_invs (fst W)\<close>
-      apply (rule twl_struct_invs_init_twl_struct_invs)
-      using snd_T struct_invs T_V V_W
-      by (auto simp: twl_st_init twl_st_l_init twl_st_wl_init)
-    obtain M N NE Q Wa UE where
-      S\<^sub>0: \<open>T = ((M, N, None, NE, UE, Q, Wa), {#})\<close>
-      using confl snd_T T_T'
-      by (cases T) (auto simp: clauses_def mset_take_mset_drop_mset' added_only_watched_def)
-    have learned_U:
-      \<open>learned_clss_lf (get_clauses_l_init U) = {#}\<close>
-      \<open>get_clauses_l_init U = fmempty\<close>
-      \<open>other_clauses_l_init U  = {#}\<close>
-      \<open>get_unit_clauses_l_init U = {#}\<close>
-      using U T_V V_W T_T'
-      by (cases U; auto simp: state_wl_l_init_def state_wl_l_def
-           twl_st_l_init_def added_only_watched_def state_wl_l_init'_def; fail)+
-    then have learned_W:
-      \<open>get_learned_clauses_init W = {#}\<close> \<open>get_unit_learned_clauses_init W = {#}\<close>
-      \<open>get_unit_init_clauses_init W = get_unit_clauses_l_init V\<close>
-      using U T_V V_W learned learned_UV by (cases T; cases U; cases V;
-         auto simp: state_wl_l_init_def state_wl_l_def twl_st_l_init_def; fail)+
-    then have [simp]: \<open>UE = {#}\<close>
-      using T_V V_W T_T' unfolding S\<^sub>0
-      by (auto simp: state_wl_l_init_def state_wl_l_def twl_st_l_init_def
-        added_only_watched_def state_wl_l_init'_def)
-    have st:
-      \<open>get_unit_clauses_l_init V = NE\<close>
-      \<open>get_clauses_l_init V = N\<close>
-      \<open>other_clauses_l_init V = {#}\<close>
-      \<open>(M, trail (state\<^sub>W_of (fst W))) \<in> convert_lits_l N (NE+UE)\<close>
-      \<open>get_trail_l_init V = M\<close>
-      \<open>cdcl\<^sub>W_restart_mset.clauses (state\<^sub>W_of (fst W)) = mset `# (ran_mf N) + NE\<close>
-      using T_V V_W T_T' unfolding S\<^sub>0
-      by (auto simp: state_wl_l_init_def state_wl_l_def twl_st_l_init_def
-          mset_take_mset_drop_mset mset_take_mset_drop_mset' clauses_def
-          added_only_watched_def state_wl_l_init'_def
-          simp del: all_clss_l_ran_m
-          simp: all_clss_lf_ran_m[symmetric])
-    have N_NE: \<open>mset `# ran_mf N + NE = mset `# mset CS'\<close>
-      \<open>{#mset (fst x). x \<in># ran_m N#} + NE  = mset `# mset CS'\<close>
-      using clss T_V V_W learned_U
-      by (auto simp: clauses_def mset_take_mset_drop_mset' S\<^sub>0 st)
-    have \<L>\<^sub>a\<^sub>l\<^sub>l_NNUE: \<open>set_mset (\<L>\<^sub>a\<^sub>l\<^sub>l (all_atms N NE)) = set_mset (all_lits_of_mm (mset `# mset CS'))\<close>
-      unfolding \<L>\<^sub>a\<^sub>l\<^sub>l_def N_NE all_atms_def all_lits_def all_lits_of_mm_def
-      by auto
-       
-    define MW where \<open>MW = trail (state\<^sub>W_of (fst W))\<close>
-    have st_W: \<open>state\<^sub>W_of (fst W) = (MW, mset `# mset CS', {#}, None)\<close>
-      using T_V V_W learned_UV learned_U clss st T_T' unfolding S\<^sub>0
-      by (auto simp: state_wl_l_init_def state_wl_l_def twl_st_l_init_def
-          mset_take_mset_drop_mset mset_take_mset_drop_mset' clauses_def MW_def
-          added_only_watched_def state_wl_l_init'_def
-          simp del: all_clss_l_ran_m
-          simp: all_clss_lf_ran_m[symmetric])
-    have n_d: \<open>no_dup MW\<close> and
-      propa: \<open>\<And>L mark a b. a @ Propagated L mark # b = MW \<Longrightarrow>
-            b \<Turnstile>as CNot (remove1_mset L mark) \<and> L \<in># mark\<close> and
-      clss_in_clss: \<open>set (get_all_mark_of_propagated MW) \<subseteq> set_mset (mset `# mset CS')\<close>
-      using struct_invs unfolding twl_struct_invs_def S\<^sub>0 twl_struct_invs_init_def
-          cdcl\<^sub>W_restart_mset.cdcl\<^sub>W_all_struct_inv_def cdcl\<^sub>W_restart_mset.cdcl\<^sub>W_conflicting_def
-          cdcl\<^sub>W_restart_mset.cdcl\<^sub>W_M_level_inv_def st cdcl\<^sub>W_restart_mset.cdcl\<^sub>W_learned_clause_def
-          N_NE st_W clauses_def
-      by simp_all
-    have count_dec': \<open>\<forall>L\<in>set MW. \<not>is_decided L\<close>
-      using V_W count_dec unfolding st MW_def twl_st_init
-      apply (subst twl_st_l_init_no_decision_iff)
-       apply assumption
-      using count_dec V_W unfolding st MW_def by auto
-    have CS: \<open>CS = mset `# mset CS'\<close>
-      using CS'_CS by (auto simp: in_list_mset_rel in_list_mset_rel_mset_rel)
-    have 0: \<open>cdcl\<^sub>W_restart_mset.cdcl\<^sub>W_stgy\<^sup>*\<^sup>* ([], CS, {#}, None)
-       (MW, mset `# mset CS', {#}, None)\<close>
-      using n_d count_dec' propa clss_in_clss
-    proof (induction MW)
-      case Nil
-      then show ?case by (auto simp: CS)
-    next
-      case (Cons K MW) note IH = this(1) and H = this(2-) and n_d = this(2) and dec = this(3) and
-        propa = this(4) and clss_in_clss = this(5)
-      let ?init = \<open>([], CS, {#}, None)\<close>
-      let ?int = \<open>(MW, mset `# mset CS', {#}, None)\<close>
-      let ?final = \<open>(K # MW, mset `# mset CS', {#}, None)\<close>
-      obtain L C where
-        K: \<open>K = Propagated L C\<close>
-        using dec by (cases K) auto
-      have 1: \<open>cdcl\<^sub>W_restart_mset.cdcl\<^sub>W_stgy\<^sup>*\<^sup>* ?init ?int\<close>
-        apply (rule IH)
-        subgoal using n_d by simp
-        subgoal using dec by simp
-        subgoal for M2 L' mark M1
-          using K propa[of \<open>K # M2\<close> L' mark M1]
-          by (auto split: if_splits)
-        subgoal using clss_in_clss by (auto simp: K)
-        done
-      have \<open>MW \<Turnstile>as CNot (remove1_mset L C)\<close> and \<open>L \<in># C\<close>
-        using propa[of \<open>[]\<close> L C \<open>MW\<close>]
-        by (auto simp: K)
-      moreover have \<open>C \<in># cdcl\<^sub>W_restart_mset.clauses (MW, mset `# mset CS', {#}, None)\<close>
-        using clss_in_clss by (auto simp: K clauses_def split: if_splits)
-      ultimately have \<open>cdcl\<^sub>W_restart_mset.propagate ?int
-            (Propagated L C # MW, mset `# mset CS', {#}, None)\<close>
-        using n_d apply -
-        apply (rule cdcl\<^sub>W_restart_mset.propagate_rule[of _ \<open>C\<close> L])
-        by (auto simp: K)
-      then have 2: \<open>cdcl\<^sub>W_restart_mset.cdcl\<^sub>W_stgy ?int ?final\<close>
-        by (auto simp add: K dest!: cdcl\<^sub>W_restart_mset.cdcl\<^sub>W_stgy.propagate')
-
-      show ?case
-        apply (rule rtranclp.rtrancl_into_rtrancl[OF 1])
-        apply (rule 2)
-        .
-    qed
-    have \<L>\<^sub>a\<^sub>l\<^sub>l: \<open>is_\<L>\<^sub>a\<^sub>l\<^sub>l (mset_set (extract_atms_clss CS' {})) (all_lits_of_mm (mset `# mset CS'))\<close>
-      by (auto simp add: is_\<L>\<^sub>a\<^sub>l\<^sub>l_extract_atms_clss)
-    have [simp]: \<open>isasat_input_bounded (mset_set (extract_atms_clss CS' {}))\<close>
-      unfolding isasat_input_bounded_def
-    proof
-      fix L
-      assume L: \<open>L \<in># \<L>\<^sub>a\<^sub>l\<^sub>l (mset_set (extract_atms_clss CS' {}))\<close>
-      then obtain C where
-        L: \<open>C\<in>set CS' \<and> (L \<in>set C \<or> - L \<in> set C)\<close>
-      apply (cases L)
-      apply (auto simp: extract_atms_clss_alt_def uint_max_def nat_of_uint32_uint32_of_nat_id
-          \<L>\<^sub>a\<^sub>l\<^sub>l_def)+
-      apply (metis literal.exhaust_sel)+
-      done
-      have \<open>\<forall>C\<in>#CS. \<forall>L\<in>#C. nat_of_lit L \<le> uint_max\<close>
-        using CS_p by auto
-      then have \<open>nat_of_lit L \<le> uint_max \<or> nat_of_lit (-L) \<le> uint_max\<close>
-        using L unfolding CS by auto
-      then show \<open>nat_of_lit L \<le> uint_max\<close>
-        using L
-        by (cases L) (auto simp: CS extract_atms_clss_alt_def uint_max_def)
-    qed
-    have T_V': \<open>(fst T, fst V) \<in> state_wl_l None\<close>
-      using T_V T_T' by (auto simp: S\<^sub>0 state_wl_l_def state_wl_l_init_def
-        added_only_watched_def state_wl_l_init'_def)
-    have V_W': \<open>(fst V, fst W) \<in> twl_st_l None\<close>
-      using V_W by (auto simp: S\<^sub>0 twl_st_l_init_def twl_st_l_def)
-    have valid_blits: \<open>\<And>L x. x\<in>set (Wa L) \<Longrightarrow>
-           case x of (i, K, _) \<Rightarrow> K \<in># all_lits_of_mm (mset `# mset CS')\<close>
-      using corr_w unfolding correct_watching_init.simps st
-      by (auto simp: st N_NE \<L>\<^sub>a\<^sub>l\<^sub>l S\<^sub>0 literals_are_\<L>\<^sub>i\<^sub>n_def
-        blits_in_\<L>\<^sub>i\<^sub>n_def correct_watching.simps
-        all_blits_are_in_problem_init.simps
-        state_wl_l_def  correct_watching_init.simps in_\<L>\<^sub>a\<^sub>l\<^sub>l_extract_atms_clss_in_all_lits_of_mm)
-    have \<open>cdcl_twl_stgy_prog_l_pre (fst V) (fst W)\<close>
-      unfolding cdcl_twl_stgy_prog_l_pre_def
-      using V_W' struct_invs corr_w add_invs clss confl clss stgy_invs confl T_V clss_upd T_T'
-      by (auto simp: twl_st_init twl_st_l_init twl_st_wl_init)
-
-    then have \<open>cdcl_twl_stgy_prog_wl_pre (fst T) (fst W)\<close>
-      unfolding cdcl_twl_stgy_prog_wl_pre_def apply -
-      apply (rule exI[of _ \<open>fst V\<close>])
-      using T_V' corr_w by (simp add: correct_watching_init_correct_watching)
-    then have 1: \<open>cdcl_twl_stgy_prog_wl_D_pre (fst T) (fst W)\<close>
-      unfolding cdcl_twl_stgy_prog_wl_D_pre_def
-        cdcl_twl_stgy_prog_wl_pre_def
-      by (auto simp: st N_NE \<L>\<^sub>a\<^sub>l\<^sub>l S\<^sub>0 literals_are_\<L>\<^sub>i\<^sub>n_def
-        blits_in_\<L>\<^sub>i\<^sub>n_def correct_watching.simps
-        all_blits_are_in_problem_init.simps in_\<L>\<^sub>a\<^sub>l\<^sub>l_extract_atms_clss_in_all_lits_of_mm
-        state_wl_l_def correct_watching_init.simps  \<L>\<^sub>a\<^sub>l\<^sub>l_NNUE
-        dest!: valid_blits)
-    have 2:\<open>cdcl_twl_stgy_restart_prog_wl_D (from_init_state T)
-            \<le> \<Down> (state_wl_l None O twl_st_l None)
-                 (conclusive_TWL_run (fst W))\<close>
-      apply (rule cdcl_twl_stgy_restart_prog_wl_D_spec_final)
-      using CS_p \<L>\<^sub>a\<^sub>l\<^sub>l struct_invs corr_w add_invs clss confl clss
-      by (auto simp: from_init_state_def st 1)
-
-    have conclusive_le: \<open>(conclusive_TWL_run (fst W)) \<le> \<Down> ({(S', S). S = state\<^sub>W_of S'}) ?Spec\<close>
-      unfolding conc_fun_RES conclusive_TWL_run_def less_eq_nres.simps
-    proof
-      fix x
-      assume \<open>x \<in> {T. \<exists>n n'.
-             cdcl_twl_stgy_restart_with_leftovers\<^sup>*\<^sup>* (fst W, n) (T, n') \<and> final_twl_state T}\<close>
-      then obtain n n' where
-        twl: \<open>cdcl_twl_stgy_restart_with_leftovers\<^sup>*\<^sup>* (fst W, n) (x, n')\<close> and
-       final: \<open>final_twl_state x\<close>
-        by blast+
-      have \<open>cdcl\<^sub>W_restart_mset.cdcl\<^sub>W_restart_stgy\<^sup>*\<^sup>* (state\<^sub>W_of (fst W), n) (state\<^sub>W_of x, n')\<close>
-        using rtranclp_cdcl_twl_stgy_restart_with_leftovers_cdcl\<^sub>W_restart_stgy[OF twl] struct_invs
-          stgy_invs by simp
-      with cdcl\<^sub>W_restart_mset.rtranclp_cdcl\<^sub>W_stgy_cdcl\<^sub>W_restart_stgy[OF 0, of n]
-      have stgy: \<open>cdcl\<^sub>W_restart_mset.cdcl\<^sub>W_restart_stgy\<^sup>*\<^sup>* (([], mset `# mset CS', {#}, None), n)
-            (state\<^sub>W_of x, n')\<close>
-        unfolding st_W CS by simp
-      have struct_invs_x: \<open>twl_struct_invs x\<close>
-        using twl struct_invs rtranclp_cdcl_twl_stgy_restart_with_leftovers_twl_struct_invs[OF twl]
-        by simp
-      then have all_struct_invs_x: \<open>cdcl\<^sub>W_restart_mset.cdcl\<^sub>W_all_struct_inv (state\<^sub>W_of x)\<close>
-        unfolding twl_struct_invs_def
-        by blast
-
-      have M_lev: \<open>cdcl\<^sub>W_restart_mset.cdcl\<^sub>W_M_level_inv ([], mset `# mset CS', {#}, None)\<close>
-        by (auto simp: cdcl\<^sub>W_restart_mset.cdcl\<^sub>W_M_level_inv_def)
-
-      have learned: \<open>cdcl\<^sub>W_restart_mset.cdcl\<^sub>W_learned_clause ([], mset `# mset CS', {#}, None)\<close>
-        unfolding cdcl\<^sub>W_restart_mset.cdcl\<^sub>W_all_struct_inv_def cdcl\<^sub>W_restart_mset.cdcl\<^sub>W_learned_clause_def
-        by auto
-      have ent: \<open>cdcl\<^sub>W_restart_mset.cdcl\<^sub>W_learned_clauses_entailed_by_init ([], mset `# mset CS', {#}, None)\<close>
-        by (auto simp: cdcl\<^sub>W_restart_mset.cdcl\<^sub>W_learned_clauses_entailed_by_init_def)
-
-      have [simp]: \<open>CS' \<noteq> []\<close>
-        using CS'_nempty by (auto simp: CS)
-
-      have entailed: \<open>cdcl\<^sub>W_restart_mset.cdcl\<^sub>W_learned_clauses_entailed_by_init (state\<^sub>W_of x)\<close>
-        apply (rule cdcl\<^sub>W_restart_mset.rtranclp_cdcl\<^sub>W_learned_clauses_entailed)
-           apply (rule cdcl\<^sub>W_restart_mset.rtranclp_cdcl\<^sub>W_restart_stgy_cdcl\<^sub>W_restart[OF stgy, unfolded fst_conv])
-          apply (rule learned)
-         apply (rule M_lev)
-        apply (rule ent)
-        done
-
-
-      consider
-        (ns) \<open>no_step cdcl_twl_stgy x\<close> |
-        (stop) \<open>get_conflict x \<noteq> None\<close> and \<open>count_decided (get_trail x) = 0\<close>
-        using final unfolding final_twl_state_def by auto
-      then show \<open>x \<in> {(S', S). S = state\<^sub>W_of S'}\<inverse> ``
-          Collect(conclusive_CDCL_run CS (init_state CS) )\<close>
-      proof cases
-        case ns
-        from no_step_cdcl_twl_stgy_no_step_cdcl\<^sub>W_stgy[OF this]
-        have \<open>no_step cdcl\<^sub>W_restart_mset.cdcl\<^sub>W (state\<^sub>W_of x)\<close>
-          using struct_invs struct_invs_x by (blast dest: cdcl\<^sub>W_ex_cdcl\<^sub>W_stgy)
-        then show ?thesis
-          using twl stgy
-          unfolding conclusive_CDCL_run_def
-          by (auto simp: CS)
-      next
-        case stop
-        have \<open>unsatisfiable (set_mset (init_clss (state\<^sub>W_of x)))\<close>
-          apply (rule conflict_of_level_unsatisfiable)
-             apply (rule all_struct_invs_x)
-          using entailed stop by (auto simp: twl_st)
-        then have \<open>unsatisfiable (mset ` set CS')\<close>
-          using cdcl\<^sub>W_restart_mset.rtranclp_cdcl\<^sub>W_restart_init_clss[symmetric, OF
-             cdcl\<^sub>W_restart_mset.rtranclp_cdcl\<^sub>W_restart_stgy_cdcl\<^sub>W_restart[OF stgy]]
-          by auto
-
-        then show ?thesis
-          using stop
-          by (auto simp: CS twl_st_init twl_st conclusive_CDCL_run_def)
-      qed
-    qed
-    show ?steps
-      unfolding TWL_to_clauses_state_conv_def from_init_state_def[symmetric]
-      apply (rule order_trans)
-       apply (rule 2)
-      apply (subst (2) conc_fun_chain[symmetric])
-      apply (rule ref_two_step)
-       prefer 2
-       apply (rule conclusive_le)
-      apply simp
-      done
-    show ?clss
-      using clss U unfolding all_clss_lf_ran_m
-      by (cases U)
-        (auto simp: S\<^sub>0 state_wl_l_init_def state_wl_l_def N_NE)
-
-    have 2:\<open>cdcl_twl_stgy_restart_prog_wl_D (from_init_state T)
-            \<le> \<Down> (state_wl_l None O twl_st_l None)
-                 (conclusive_TWL_run (fst W))\<close>
-      apply (rule cdcl_twl_stgy_restart_prog_wl_D_spec_final)
-      using CS_p \<L>\<^sub>a\<^sub>l\<^sub>l
-        struct_invs corr_w add_invs clss confl clss
-      by (auto simp: from_init_state_def st 1)
-    show ?break_steps
-      unfolding TWL_to_clauses_state_conv_def from_init_state_def[symmetric]
-      apply (rule order_trans)
-       apply (rule 2)
-      apply (subst (2) conc_fun_chain[symmetric])
-      apply (rule ref_two_step)
-       prefer 2
-       apply (rule conclusive_le)
-      by simp
-    show ?learned_clss
-      using learned_U learned_UV T_V T_T'
-      by (cases T, cases V) (auto simp: state_wl_l_init_def state_wl_l_def
-        added_only_watched_def state_wl_l_init'_def)
-  qed
-
-  have init: \<open>init_dt_wl_pre CS' (([], fmempty, None, {#}, {#}, {#}), {#})\<close>
-    if \<open>Ball (set CS') distinct\<close> for CS'
-    using that
-    by (auto simp: init_dt_wl_pre_def init_dt_pre_def state_wl_l_init_def
-        twl_st_l_init_def state_wl_l_def correct_watching_init.simps clause_to_update_def
-        twl_init_invs all_blits_are_in_problem_init.simps
-        state_wl_l_init'_def)
-
-  have [simp]: \<open>finite (extract_atms_clss CS' {})\<close> for CS'
-    by  (auto simp: extract_atms_clss_alt_def)
-
-  have K: \<open>mset_set (extract_atms_clss CS' {}) = {#} \<longleftrightarrow> (\<forall>C \<in>set CS'. C = [])\<close> for CS'
-    by  (auto simp: extract_atms_clss_alt_def mset_set_empty_iff)
-  then have K'[dest]: \<open>x \<in> (extract_atms_clss CS' {}) \<Longrightarrow> \<not>(\<forall>C \<in>set CS'. C = [])\<close> for CS' x
-    using K[of CS'] by (auto simp:  mset_set_empty_iff)
-  show ?thesis
-    unfolding SAT_wl_def SAT_def from_init_state_def to_init_state_def
-      empty_watched_def finalise_init_def id_def
-    apply (intro frefI nres_relI)
-    subgoal for CS' CS
-      apply (rewrite at \<open>let _ = extract_atms_clss _ _ in _\<close> Let_def)
-      apply (simp only: if_False init_state_wl_def empty_watched_def)
-      apply (refine_vcg  (* bind_refine_spec*) lhs_step_If init_dt_wl_init_dt_wl_spec
-         bind_refine_spec[OF _ init_dt_wl_full_init_dt_wl_spec_full]
-	 bind_refine_res[OF _ init_dt_wl'_spec[unfolded conc_fun_RES]])
-	 thm bind_refine_spec[OF _ init_dt_wl_full_init_dt_wl_spec_full]
-	 find_theorems init_dt_wl'
-      \<comment> \<open>First the fast part:\<close>
-      subgoal for b by (rule conflict_during_init)
-      subgoal for T by (rule empty_clss)
-      subgoal by (rule extract_atms_clss_not_nil)
-      subgoal by (auto simp: in_list_mset_rel in_list_mset_rel_mset_rel K
-         isasat_input_bounded_nempty_def isasat_input_bounded_nempty_axioms_def)
-      subgoal by (rule clauses)
-      subgoal by (rule learned_clss)
-      subgoal by (rule break_CDCL_steps)
-      subgoal by (rule init) (auto simp: in_list_mset_rel in_list_mset_rel_mset_rel)
-(*       \<comment> \<open>Now the slow part: \<close>
-      subgoal for b by (rule conflict_during_init)
-      subgoal for T by (rule empty_clss)
-      subgoal by (rule extract_atms_clss_not_nil)
-      subgoal by (auto simp: in_list_mset_rel in_list_mset_rel_mset_rel K
-         isasat_input_bounded_nempty_def isasat_input_bounded_nempty_axioms_def)
-      subgoal by (rule clauses)
-      subgoal by (rule learned_clss)
-      subgoal by (rule CDCL_steps)
-      subgoal by (rule init) (auto simp: in_list_mset_rel in_list_mset_rel_mset_rel) *)
-      done
-    done
-qed
 
 definition model_if_satisfiable :: \<open>nat clauses \<Rightarrow> nat literal list option nres\<close> where
   \<open>model_if_satisfiable CS = SPEC (\<lambda>M.
@@ -3039,6 +2745,139 @@ lemma SAT_model_if_satisfiable':
     [\<lambda>(_, CS). (\<forall>C \<in># CS. distinct_mset C)]\<^sub>f Id \<times>\<^sub>r Id\<rightarrow> \<langle>Id\<rangle>nres_rel\<close>
   using SAT_model_if_satisfiable by (auto simp: fref_def)
 
+definition SAT_l' where
+  \<open>SAT_l' CS = do{
+    S \<leftarrow> SAT_l CS;
+    RETURN (if get_conflict_l S = None then Some (map lit_of (get_trail_l S)) else None)
+  }\<close>
+
+
+definition SAT0' where
+  \<open>SAT0' CS = do{
+    S \<leftarrow> SAT0 CS;
+    RETURN (if get_conflict S = None then Some (map lit_of (get_trail S)) else None)
+  }\<close>
+
+
+lemma twl_st_l_map_lit_of[twl_st_l, simp]:
+  \<open>(S, T) \<in> twl_st_l b \<Longrightarrow> map lit_of (get_trail_l S) = map lit_of (get_trail T)\<close>
+  by (auto simp: twl_st_l_def convert_lits_l_map_lit_of)
+  
+
+lemma ISASAT_SAT_l':
+  assumes \<open>Multiset.Ball (mset `# mset CS) distinct_mset\<close> and
+    \<open>isasat_input_bounded (mset_set (\<Union>C\<in>set CS. atm_of ` set C))\<close>
+  shows \<open>IsaSAT CS \<le> \<Down> Id (SAT_l' CS)\<close>
+  unfolding IsaSAT_def SAT_l'_def
+  apply refine_vcg
+  apply (rule SAT_wl_SAT_l)
+  subgoal using assms by auto
+  subgoal using assms by auto
+  subgoal by (auto simp: extract_model_of_state_def)
+  done
+
+lemma SAT_l'_SAT0':
+  assumes \<open>Multiset.Ball (mset `# mset CS) distinct_mset\<close>
+  shows \<open>SAT_l' CS \<le> \<Down> Id (SAT0' CS)\<close>
+  unfolding SAT_l'_def SAT0'_def
+  apply refine_vcg
+  apply (rule SAT_l_SAT0)
+  subgoal using assms by auto
+  subgoal by (auto simp: extract_model_of_state_def)
+  done
+
+lemma SAT0'_SAT':
+  assumes \<open>Multiset.Ball (mset `# mset CS) distinct_mset\<close>
+  shows \<open>SAT0' CS \<le> \<Down> Id (SAT' (mset `# mset CS))\<close>
+  unfolding SAT'_def SAT0'_def
+  apply refine_vcg
+  apply (rule SAT0_SAT)
+  subgoal using assms by auto
+  subgoal by (auto simp: extract_model_of_state_def twl_st_l twl_st)
+  done
+
+
+lemma IsaSAT_heur_model_if_sat:
+  assumes \<open>\<forall>C \<in># mset `# mset CS. distinct_mset C\<close> and
+    \<open>isasat_input_bounded (mset_set (\<Union>C\<in>set CS. atm_of ` set C))\<close>
+  shows \<open>IsaSAT_heur opts CS \<le> \<Down> model_stat_rel (model_if_satisfiable (mset `# mset CS))\<close>
+  apply (rule IsaSAT_heur_IsaSAT[THEN order_trans])
+  apply (rule order_trans)
+  apply (rule ref_two_step')
+  apply (rule ISASAT_SAT_l')
+  subgoal using assms by auto
+  subgoal using assms by auto
+
+  unfolding conc_fun_chain
+  apply (rule order_trans)
+  apply (rule ref_two_step')
+  apply (rule SAT_l'_SAT0')
+  subgoal using assms by auto
+
+  unfolding conc_fun_chain
+  apply (rule order_trans)
+  apply (rule ref_two_step')
+  apply (rule SAT0'_SAT')
+  subgoal using assms by auto
+
+  unfolding conc_fun_chain
+  apply (rule order_trans)
+  apply (rule ref_two_step')
+  apply (rule SAT_model_if_satisfiable[THEN fref_to_Down, of \<open>mset `# mset CS\<close>])
+  subgoal using assms by auto
+  subgoal using assms by auto
+
+  unfolding conc_fun_chain
+  apply (rule conc_fun_R_mono)
+  apply (auto simp: model_stat_rel_def)
+  done
+
+lemma IsaSAT_heur_model_if_sat': \<open>(uncurry IsaSAT_heur, uncurry (\<lambda>_. model_if_satisfiable)) \<in>
+   [\<lambda>(_, CS). (\<forall>C \<in># CS. distinct_mset C) \<and>
+     (\<forall>C\<in>#CS. \<forall>L\<in>#C. nat_of_lit L \<le> uint_max)]\<^sub>f
+     Id \<times>\<^sub>r list_mset_rel O \<langle>list_mset_rel\<rangle>mset_rel \<rightarrow> \<langle>model_stat_rel\<rangle>nres_rel\<close>
+proof -
+  have H: \<open>isasat_input_bounded (mset_set (\<Union>C\<in>set CS. atm_of ` set C))\<close>
+    if CS_p: \<open>\<forall>C\<in>#CS'. \<forall>L\<in>#C. nat_of_lit L \<le> uint_max\<close> and
+      \<open>(CS, CS') \<in> list_mset_rel O \<langle>list_mset_rel\<rangle>mset_rel\<close>
+    for CS CS'
+    unfolding isasat_input_bounded_def
+  proof
+    fix L
+    assume L: \<open>L \<in># \<L>\<^sub>a\<^sub>l\<^sub>l (mset_set (\<Union>C\<in>set CS. atm_of ` set C))\<close>
+    then obtain C where
+      L: \<open>C\<in>set CS \<and> (L \<in>set C \<or> - L \<in> set C)\<close>
+      apply (cases L)
+      apply (auto simp: extract_atms_clss_alt_def uint_max_def nat_of_uint32_uint32_of_nat_id
+          \<L>\<^sub>a\<^sub>l\<^sub>l_def)+
+      apply (metis literal.exhaust_sel)+
+      done
+    have \<open>nat_of_lit L \<le> uint_max \<or> nat_of_lit (-L) \<le> uint_max\<close>
+      using L CS_p that by (auto simp: list_mset_rel_def mset_rel_def br_def
+      br_def mset_rel_def p2rel_def rel_mset_def
+        rel2p_def[abs_def] list_all2_op_eq_map_right_iff')
+    then show \<open>nat_of_lit L \<le> uint_max\<close>
+      using L
+      by (cases L) (auto simp: extract_atms_clss_alt_def uint_max_def)
+  qed
+  show ?thesis
+    apply (intro frefI nres_relI)
+    unfolding uncurry_def
+    apply clarify
+    subgoal for o1 o2 o3 CS o1' o2' o3' CS'
+    apply (rule IsaSAT_heur_model_if_sat[THEN order_trans, of CS _ \<open>(o1, o2, o3)\<close>])
+    subgoal by (auto simp: list_mset_rel_def mset_rel_def br_def
+      br_def mset_rel_def p2rel_def rel_mset_def
+        rel2p_def[abs_def] list_all2_op_eq_map_right_iff')
+    subgoal by (rule H) auto
+    apply (auto simp: list_mset_rel_def mset_rel_def br_def
+      br_def mset_rel_def p2rel_def rel_mset_def
+        rel2p_def[abs_def] list_all2_op_eq_map_right_iff')
+    done
+    done
+qed
+
+
 lemma list_assn_list_mset_rel_clauses_l_assn:
   \<open>(hr_comp (list_assn (list_assn unat_lit_assn)) (list_mset_rel O \<langle>list_mset_rel\<rangle>mset_rel)) xs xs'
      = clauses_l_assn xs xs'\<close>
@@ -3064,430 +2903,15 @@ proof -
         simp del: literal_of_nat.simps)
 qed
 
-lemma twl_st_heur_init_vmtf_next_emptyD:
-  \<open>((x1, x1a, x1b, x1c, x1d, ((x1g, x1h, x1i, x1j, x2h), x2i), x1k, x2k), Ta)
-       \<in> twl_st_heur_parsing \<A>\<^sub>i\<^sub>n \<Longrightarrow> \<A>\<^sub>i\<^sub>n \<noteq> {#} \<Longrightarrow> x1i \<noteq> None\<close>
-  by (auto simp: twl_st_heur_parsing_def vmtf_init_def isa_vmtf_init_def)
 
-lemma twl_st_heur_init_vmtf_fstD:
-  \<open>((x1, x1a, x1b, x1c, x1d, ((x1g, x1h, x1i, x1j, x2h), x2i), x1k, x2k), Ta)
-       \<in> twl_st_heur_parsing \<A>\<^sub>i\<^sub>n \<Longrightarrow> \<A>\<^sub>i\<^sub>n \<noteq> {#} \<Longrightarrow> x1j \<noteq> None\<close>
-  by (auto simp: twl_st_heur_parsing_def vmtf_init_def isa_vmtf_init_def)
-
-(* 
-lemma get_conflict_wl_is_None_init_get_conflict_wl_is_None_heur_init[simp]:
-  \<open>(Tb, Ta) \<in> twl_st_heur_parsing A \<Longrightarrow>
-     get_conflict_wl_is_None_init (from_init_state Ta) = get_conflict_wl_is_None_heur_init Tb\<close>
-  by (cases Ta; cases Tb)
-    (auto simp: from_init_state_def
-      get_conflict_wl_is_None_init_def get_conflict_wl_is_None_heur_init_def
-      isasat_input_ops.twl_st_heur_parsing_def isasat_input_ops.option_lookup_clause_rel_def
-      get_conflict_wl_is_None_def split: option.splits)
-
-
-lemma(in isasat_input_ops) get_clauses_wl_from_init_get_clauses_wl_heur_init:
-  \<open>(T, Ta) \<in> twl_st_heur_init \<Longrightarrow> get_clauses_wl (from_init_state Ta) = get_clauses_wl_heur_init T\<close>
-  by (cases T; cases Ta)
-    (auto simp: twl_st_heur_init_def twl_st_heur_init_wl_def from_init_state_def)
-
-lemma isasat_input_bounded_nempty_cdcl_twl_stgy_prog_wl_D_heur_break_cdcl_twl_stgy_prog_wl_D':
-  \<open>isasat_input_bounded_nempty \<A> \<Longrightarrow> (S, S') \<in> isasat_input_ops.twl_st_heur \<A> \<Longrightarrow> \<A> = \<A>' \<Longrightarrow>
-   isasat_input_ops.cdcl_twl_stgy_prog_break_wl_D_heur_break \<A> S
-    \<le> \<Down> (isasat_input_ops.twl_st_heur \<A>)
-         (isasat_input_ops.cdcl_twl_stgy_prog_break_wl_D \<A>' S')\<close>
-  using isasat_input_bounded_nempty.cdcl_twl_stgy_prog_wl_D_heur_break_cdcl_twl_stgy_prog_wl_D
-             [THEN fref_to_Down, unfolded comp_def, of \<A> S S']
-  by fast *)
-
-lemma isasat_input_bounded_nempty_cdcl_twl_stgy_restart_prog_wl_D_heur_break_cdcl_twl_stgy_prog_wl_D':
-  \<open>isasat_input_bounded_nempty \<A> \<Longrightarrow> (S, S') \<in> twl_st_heur \<Longrightarrow> \<A> = \<A>' \<Longrightarrow>
-    cdcl_twl_stgy_restart_prog_wl_heur S
-    \<le> \<Down>(twl_st_heur)
-         (cdcl_twl_stgy_restart_prog_wl_D S')\<close>
-  using cdcl_twl_stgy_restart_prog_wl_heur_cdcl_twl_stgy_restart_prog_wl_D
-             [THEN fref_to_Down, unfolded comp_def, of S S']
-  by fast
-
-lemma IsaSAT_heur_IsaSAT: \<open>(uncurry IsaSAT_heur, uncurry (\<lambda>_. IsaSAT)) \<in>
-     [\<lambda>(_, CS). Multiset.Ball (mset CS) distinct \<and> (\<forall>C\<in>set CS. \<forall>L\<in>set C. nat_of_lit L \<le> uint_max)]\<^sub>f
-     Id \<times>\<^sub>r Id \<rightarrow> \<langle>{((M, stat), M'). map_option rev M = M'}\<rangle>nres_rel\<close>
-proof -
-  have H: \<open>A + B = C \<Longrightarrow> A \<subseteq># C\<close> for A B C
-    by auto
-  define f :: \<open>twl_st_wl_heur_init \<Rightarrow> twl_st_wl_heur_init nres\<close> where \<open>f = RETURN\<close>
-  have IsaSAT_heur_alt_def: \<open>IsaSAT_heur opts CS = do{
-    ASSERT(\<forall>C\<in>set CS. \<forall>L\<in>set C. nat_of_lit L \<le> uint_max);
-    let \<A>\<^sub>i\<^sub>n'' = mset_set (extract_atms_clss CS {});
-    ASSERT(isasat_input_bounded \<A>\<^sub>i\<^sub>n'');
-    ASSERT(distinct_mset \<A>\<^sub>i\<^sub>n'');
-    let b = False;
-    \<^cancel>\<open>if b \<and> length CS < uint_max - 1
-    then do {
-        S \<leftarrow> isasat_input_ops.init_state_wl_heur \<A>\<^sub>i\<^sub>n'';
-        S \<leftarrow> f S;
-        (T::twl_st_wl_heur_init) \<leftarrow> isasat_input_ops.init_dt_wl_heur \<A>\<^sub>i\<^sub>n'' CS S;
-        if \<not>get_conflict_wl_is_None_heur_init T
-        then RETURN (empty_init_code)
-        else if CS = [] then empty_conflict_code
-        else do {
-           ASSERT(\<A>\<^sub>i\<^sub>n'' \<noteq> {#});
-           ASSERT(isasat_input_bounded_nempty \<A>\<^sub>i\<^sub>n'');
-           ASSERT((\<lambda>(M', N', D', Q', W', ((ns, m, fst_As, lst_As, next_search), to_remove), \<phi>, clvls). fst_As \<noteq> None \<and>
-             lst_As \<noteq> None) T);
-           T \<leftarrow> finalise_init_code (T::twl_st_wl_heur_init);
-           ASSERT(isasat_fast T);
-           U \<leftarrow> isasat_input_ops.cdcl_twl_stgy_prog_wl_D_heur \<A>\<^sub>i\<^sub>n'' T;
-           RETURN (if get_conflict_wl_is_None_heur U then extract_model_of_state_stat U
-             else extract_state_stat U)
-         }
-      }
-    else\<close>
-        S \<leftarrow> init_state_wl_heur;
-        S \<leftarrow> f S;
-        (T::twl_st_wl_heur_init) \<leftarrow> init_dt_wl_heur_full CS S;
-        if \<not>get_conflict_wl_is_None_heur_init T
-        then RETURN (empty_init_code)
-        else if CS = [] then empty_conflict_code
-        else do {
-           ASSERT(\<A>\<^sub>i\<^sub>n'' \<noteq> {#});
-           ASSERT(isasat_input_bounded_nempty \<A>\<^sub>i\<^sub>n'');
-           ASSERT((\<lambda>(M', N', D', Q', W', ((ns, m, fst_As, lst_As, next_search), to_remove), \<phi>, clvls). fst_As \<noteq> None \<and>
-             lst_As \<noteq> None) T);
-           T \<leftarrow> finalise_init_code opts (T::twl_st_wl_heur_init);
-           U \<leftarrow> cdcl_twl_stgy_restart_prog_wl_heur T;
-           RETURN (if get_conflict_wl_is_None_heur U then extract_model_of_state_stat U
-             else extract_state_stat U)
-         }
-
-    }\<close>  (is \<open>?A = ?B\<close>) for CS opts
-  proof -
-    have [simp]: \<open>ASSERT \<Phi> \<bind> (\<lambda>_. P) \<le> ASSERT \<Phi> \<bind> (\<lambda>_. Q) \<longleftrightarrow> (\<Phi> \<longrightarrow> P \<le> Q)\<close> for \<Phi> P Q
-      using Refine_Basic.le_ASSERTI_pres by auto
-
-    have 1: \<open>?A \<le> ?B\<close>
-      unfolding IsaSAT_heur_def Let_def isasat_input_ops.init_state_wl_heur_fast_def f_def
-        empty_conflict_code_def empty_conflict_code_def empty_init_code_def convert_state_def
-        isasat_information_banner_def
-      apply (refine_vcg lhs_step_If)
-       apply (auto intro!:  Refine_Basic.bind_mono)
-      (* apply (subst isasat_input_ops.init_dt_wl_heur_fast_init_dt_wl_heur)
-      apply (auto simp: isasat_input_ops.init_state_wl_heur_def map_fun_rel_def
-          RES_RES_RETURN_RES RETURN_def in_class_in_literals_are_in_\<L>\<^sub>i\<^sub>n Max_dom_fmempty) *)
-      done
-
-    have 2: \<open>?B \<le> ?A\<close>
-      unfolding IsaSAT_heur_def Let_def isasat_input_ops.init_state_wl_heur_fast_def f_def
-        empty_conflict_code_def empty_conflict_code_def empty_init_code_def convert_state_def
-        isasat_information_banner_def
-      apply (refine_vcg lhs_step_If)
-      apply (auto intro!:  Refine_Basic.bind_mono)
-      (* apply (subst isasat_input_ops.init_dt_wl_heur_fast_init_dt_wl_heur)
-      apply (auto simp: isasat_input_ops.init_state_wl_heur_def map_fun_rel_def
-          RES_RES_RETURN_RES RETURN_def in_class_in_literals_are_in_\<L>\<^sub>i\<^sub>n Max_dom_fmempty) *)
-      done
-    show ?thesis using 1 2 by simp
-  qed
-
-  have [refine]: \<open>inres
-        (isasat_input_ops.init_state_wl_heur
-          (mset_set (extract_atms_clss x {})))
-        S \<Longrightarrow>
-       (S, isasat_input_ops.init_state_wl)
-       \<in> isasat_input_ops.twl_st_heur_parsing_no_WL_wl N \<Longrightarrow>
-       f S
-       \<le> \<Down> {(T, (T', OS)). (T, (T', OS)) \<in> isasat_input_ops.twl_st_heur_parsing_no_WL N}
-          (RETURN (to_init_state isasat_input_ops.init_state_wl))\<close>
-    (is \<open>_ \<Longrightarrow>_ \<Longrightarrow> _ \<le> \<Down> ?init _\<close>)
-    for S T' N x
-    by (auto simp: f_def inres_def isasat_input_ops.init_state_wl_heur_def
-        RES_RETURN_RES RES_RES_RETURN_RES)
-     (auto simp: f_def to_init_state_def isasat_input_ops.twl_st_heur_parsing_no_WL_def
-      isasat_input_ops.twl_st_heur_parsing_no_WL_wl_def isasat_input_ops.init_state_wl_def)
-
-
-  have init: \<open>isasat_input_ops.init_dt_wl_heur_full (mset_set (extract_atms_clss CS {})) CS T'
-      \<le> \<Down> (isasat_input_ops.twl_st_heur_parsing (mset_set (extract_atms_clss CS' {})))
-          (init_dt_wl_full CS'
-             (to_init_state (isasat_input_ops.init_state_wl)))\<close>
-    if
-      distinct: \<open>Multiset.Ball (mset CS') distinct\<close> and
-      SS': \<open>(CS, CS') \<in> Id\<close> and
-      bounded: \<open>isasat_input_bounded (mset_set (extract_atms_clss CS' {}))\<close> and
-      TT': \<open>inres (f T) T'\<close> and
-      T': \<open>(T', to_init_state (isasat_input_ops.init_state_wl))
-        \<in> {(T, T', OS).
-          (T, (T', OS)) \<in> isasat_input_ops.twl_st_heur_parsing_no_WL (mset_set (extract_atms_clss CS' {}))}\<close>
-    for CS CS' T T'
-  proof -
-    have SS': \<open>CS = CS'\<close>
-      using SS' by auto
-    have [simp]: \<open>T = T'\<close>
-      using TT' unfolding f_def by auto
-    have H: \<open>C \<in> set CS' \<Longrightarrow> \<exists>CS'''. set CS' = insert C CS'''\<close> for C
-      by auto
-    have [simp]: \<open>C \<in> set CS' \<Longrightarrow>
-       isasat_input_ops.literals_are_in_\<L>\<^sub>i\<^sub>n (mset_set (extract_atms_clss CS' {})) (mset C)\<close> for C
-      apply (auto simp: isasat_input_ops.literals_are_in_\<L>\<^sub>i\<^sub>n_def isasat_input_ops.\<L>\<^sub>a\<^sub>l\<^sub>l_def
-          extract_atms_clss_alt_def in_all_lits_of_m_ain_atms_of_iff atm_of_eq_atm_of
-          atms_of_s_def image_image image_Un in_image_uminus_uminus[symmetric]
-          dest!: H)
-      apply (metis (no_types, lifting) image_iff literal.exhaust_sel)+
-      done
-    have pre: \<open>init_dt_wl_pre CS' (to_init_state isasat_input_ops.init_state_wl)\<close>
-      using distinct
-      unfolding init_dt_wl_pre_def init_dt_pre_def
-      by (auto simp: state_wl_l_init_def isasat_input_ops.init_state_wl_def
-        to_init_state_def state_wl_l_init'_def twl_st_l_init_def
-        twl_init_invs)
-    show ?thesis
-      unfolding SS'
-      apply (rule isasat_input_bounded.init_dt_wl_heur_full_init_dt_wl_full)
-      subgoal by (rule bounded)
-      subgoal by (rule pre)
-      subgoal using T' by (auto simp: isasat_input_ops.twl_st_heur_parsing_no_WL_wl_def)
-      subgoal using T' distinct by (auto simp: isasat_input_ops.twl_st_heur_parsing_no_WL_wl_def
-            distinct_mset_set_def)
-      subgoal using T' by (cases \<open>to_init_state isasat_input_ops.init_state_wl\<close>) simp
-      done
-  qed
-
-  have from_init_state: \<open>(T, from_init_state Ta)
-        \<in> isasat_input_ops.twl_st_heur_post_parsing_wl
-          (mset_set (extract_atms_clss y {}))\<close>
-    if
-      T_Ta: \<open>(T, Ta)
-      \<in> isasat_input_ops.twl_st_heur_parsing
-          (mset_set (extract_atms_clss y {}))\<close> and
-      \<open>\<not> \<not> get_conflict_wl_is_None_heur_init T\<close>
-    for T Ta x y Sa b
-  proof -
-    show ?thesis
-      using T_Ta
-      unfolding f_def
-      by (auto simp: isasat_input_ops.twl_st_heur_parsing_def from_init_state_def
-         isasat_input_ops.twl_st_heur_post_parsing_wl_def )
-        (metis set_mset_mset)+
-  qed
-  have finalise_init: \<open>get_conflict_wl y = None \<Longrightarrow> \<A> \<noteq> {#} \<Longrightarrow> size (learned_clss_l (get_clauses_wl y)) = 0 \<Longrightarrow>
-    (y', y) \<in> isasat_input_ops.twl_st_heur_post_parsing_wl \<A> \<Longrightarrow>
-    finalise_init_code x' y' \<le> \<Down> (isasat_input_ops.twl_st_heur \<A>) (RETURN (finalise_init y))\<close>
-    for y x' y'  \<A>
-    by (rule isasat_input_ops.finalise_init_finalise_init[THEN fref_to_Down_curry, unfolded comp_def]) auto
-
-  show ?thesis
-    supply RETURN_as_SPEC_refine[refine2 del]
-    unfolding IsaSAT_heur_alt_def IsaSAT_def uncurry_def
-    apply (intro frefI nres_relI bind_refine if_refine)
-    apply (refine_vcg
-           init
-           init_state_wl_heur_init_state_wl[THEN fref_to_Down, unfolded comp_def, OF refl]
-           from_init_state
-           isasat_input_bounded_nempty.cdcl_twl_stgy_prog_wl_D_heur_cdcl_twl_stgy_prog_wl_D
-             [THEN fref_to_Down_explode, unfolded comp_def]
-           isasat_input_bounded_nempty_cdcl_twl_stgy_restart_prog_wl_D_heur_break_cdcl_twl_stgy_prog_wl_D')
-    subgoal by auto
-    subgoal by auto
-    subgoal by auto
-    subgoal by auto
-    apply (rule IdI)
-                 apply (assumption)+
-    subgoal by auto
-    subgoal by auto
-                  apply (assumption)+
-    subgoal by auto
-    subgoal by (auto simp: empty_init_code_def)
-    subgoal premises p
-      by (auto simp: empty_init_code_def)
-    subgoal by auto
-    subgoal premises p
-      by (auto simp: empty_conflict_code_def op_arl_empty_def)
-    subgoal by auto
-    subgoal by auto
-    subgoal
-      by (auto dest: isasat_input_ops.twl_st_heur_init_vmtf_next_emptyD)
-    subgoal
-      by (auto dest!: isasat_input_ops.twl_st_heur_init_vmtf_fstD)
-       apply (rule finalise_init)
-    subgoal
-      by (auto simp: get_conflict_wl_is_None_init_def get_conflict_wl_is_None_def
-          split: option.splits)
-         apply assumption+
-    apply (rule from_init_state;assumption)
-(*     subgoal for CS CS' b S' S T U' U
-      by (rule dom_m_le_uint_max)
-    subgoal by fast
-    subgoal by fast
-    subgoal premises p
-      using p(32)
-      by (auto simp: extract_model_of_state_stat_def extract_model_of_state_def
-          isasat_input_ops.twl_st_heur_def get_conflict_wl_is_None_heur_def
-          get_conflict_wl_is_None_heur_init_def extract_state_stat_def rev_map
-          get_conflict_wl_is_None_def split: option.splits)
-    subgoal by auto
-    apply assumption+
-    subgoal by fast
-    apply assumption+
-    subgoal by simp
-    subgoal premises p by (simp add: empty_init_code_def)
-    subgoal by simp
-    subgoal premises p by (simp add: empty_conflict_code_def op_arl_empty_def)
-    subgoal by auto
-    subgoal by auto
-    subgoal
-      by (auto simp: isasat_input_ops.get_clauses_wl_from_init_get_clauses_wl_heur_init
-        intro: mset_subset_eq_add_left dest: H)
-    subgoal
-      by (auto dest: isasat_input_ops.twl_st_heur_init_vmtf_next_emptyD)
-    subgoal
-      by (auto dest!: isasat_input_ops.twl_st_heur_init_vmtf_fstD)
-    subgoal
-      by (auto simp: isasat_input_ops.twl_st_heur_init_def
-        state_wl_l_def from_init_state_def)
-    subgoal
-      unfolding get_conflict_wl_is_None_init_def get_conflict_wl_is_None by meson
-    apply assumption+
-    subgoal
-      by (rule isasat_input_ops.twl_st_heur_init_wl) *)
-    subgoal by auto
-    subgoal by auto
-    subgoal premises p
-      using p(29)
-      by (auto simp: extract_model_of_state_stat_def extract_model_of_state_def
-          isasat_input_ops.twl_st_heur_def get_conflict_wl_is_None_heur_def
-          get_conflict_wl_is_None_heur_init_def extract_state_stat_def rev_map
-          isasat_input_ops.option_lookup_clause_rel_def
-          get_conflict_wl_is_None_def split: option.splits)
-    done
-qed
-
-lemma [simp]: \<open>finite (extract_atms_clss CS {})\<close>
-  by (auto simp: extract_atms_clss_alt_def)
-
-lemma IsaSAT_code: \<open>(uncurry IsaSAT_code, uncurry (\<lambda>_. SAT'))
-    \<in> [\<lambda>(_, x). Multiset.Ball x distinct_mset \<and> (\<forall>C\<in>#x. \<forall>L\<in>#C. nat_of_lit L \<le> uint_max)]\<^sub>a
-      opts_assn\<^sup>d *\<^sub>a clauses_l_assn\<^sup>k \<rightarrow> model_assn\<close>
-proof -
-  define empty_trail where
-    \<open>empty_trail = Some ([] :: nat literal list)\<close>
-  have 1: \<open>B = C \<Longrightarrow> ((A :: _ nres) \<bind> B) = ((A :: _ nres) \<bind> C)\<close> for A B C
-    by auto
-  have [simp]: \<open>mset_set (extract_atms_clss CS {}) \<noteq> {#} \<longleftrightarrow> extract_atms_clss CS {} \<noteq> {}\<close> for CS
-    using mset_set_empty_iff[of \<open>extract_atms_clss CS {}\<close>]
-    by (auto simp: )
-  have IsaSAT: \<open>IsaSAT CS = do {
-     ASSERT (isasat_input_bounded (mset_set (extract_atms_clss CS {})));
-     ASSERT (distinct_mset (mset_set (extract_atms_clss CS {})));
-     T \<leftarrow> SAT_wl CS;
-     RETURN (if get_conflict_wl T = None then extract_model_of_state T else None)
-    }\<close> for CS
-    unfolding IsaSAT_def SAT_wl_def Let_def get_conflict_wl_is_None_init_def
-     finalise_init_def id_def get_conflict_wl_is_None[symmetric] empty_trail_def
-     extract_model_of_state_def
-    by (auto cong: bind_cong simp:  intro: bind_cong intro!: 1 ext)
-
-  have 2: \<open>Multiset.Ball y distinct_mset \<Longrightarrow>
-       (x, y) \<in> list_mset_rel O \<langle>list_mset_rel\<rangle>mset_rel \<Longrightarrow>
-        (\<forall>C\<in>#y. \<forall>L\<in>#C. nat_of_lit L \<le> uint_max) \<Longrightarrow>
-       SAT_wl x \<le> \<Down> TWL_to_clauses_state_conv (SAT y)\<close> for x y
-    using cdcl_twl_stgy_prog_wl_spec_final2[unfolded fref_def nres_rel_def] by simp
-  have SAT': \<open>SAT' CS =
-       do {
-          ASSERT(True);ASSERT(True);
-          U \<leftarrow> SAT CS;
-          RETURN(if conflicting U = None then Some (map lit_of (trail U)) else None)
-      }\<close> for CS
-    unfolding SAT'_def SAT_def empty_trail_def by (auto simp: RES_RETURN_RES)
-  have 3:
-    \<open>ASSERT (isasat_input_bounded (mset_set (extract_atms_clss x {}))) \<le> \<Down> unit_rel (ASSERT True)\<close>
-    if CS_p: \<open>(\<forall>C\<in>#y. \<forall>L\<in>#C. nat_of_lit L \<le> uint_max)\<close> and
-       CS: \<open>(x, y) \<in> list_mset_rel O \<langle>list_mset_rel\<rangle>mset_rel\<close>
-       for x y
-    apply (rule ASSERT_refine)
-    unfolding isasat_input_bounded_def
-  proof
-    fix L
-    assume L: \<open>L \<in># isasat_input_ops.\<L>\<^sub>a\<^sub>l\<^sub>l (mset_set (extract_atms_clss x {}))\<close>
-    then obtain C where
-      L: \<open>C\<in>set x \<and> (L \<in>set C \<or> - L \<in> set C)\<close>
-      apply (cases L)
-      apply (auto simp: extract_atms_clss_alt_def uint_max_def nat_of_uint32_uint32_of_nat_id
-          isasat_input_ops.\<L>\<^sub>a\<^sub>l\<^sub>l_def)+
-      apply (metis literal.exhaust_sel)+
-      done
-    have \<open>\<forall>C\<in>#y. \<forall>L\<in>#C. nat_of_lit L \<le> uint_max\<close>
-      using CS_p by auto
-    then have \<open>nat_of_lit L \<le> uint_max \<or> nat_of_lit (-L) \<le> uint_max\<close>
-      using L CS by (auto simp: list_mset_rel_def br_def mset_rel_def rel2p_def[abs_def] p2rel_def
-        rel_mset_def list_all2_op_eq_map_right_iff')
-    then show \<open>nat_of_lit L \<le> uint_max\<close>
-      using L
-      by (cases L) (auto simp: extract_atms_clss_alt_def uint_max_def)
-  qed
-  have 4: \<open>ASSERT (distinct_mset (mset_set (extract_atms_clss x {}))) \<le> \<Down> unit_rel (ASSERT True)\<close>
-    for x
-    by (auto simp: distinct_mset_def)
-  have IsaSAT_SAT: \<open>(IsaSAT, SAT') \<in>
-     [\<lambda>CS. Multiset.Ball CS distinct_mset \<and>
-      (\<forall>C\<in>#CS. \<forall>L\<in>#C. nat_of_lit L \<le> uint_max)]\<^sub>f
-     list_mset_rel O \<langle>list_mset_rel\<rangle>mset_rel \<rightarrow> \<langle>\<langle>\<langle>Id\<rangle>list_rel\<rangle> option_rel\<rangle>nres_rel\<close>
-    unfolding SAT' IsaSAT
-    apply (intro frefI nres_relI bind_refine if_refine)
-         apply (rule 3; simp; fail)
-        apply (rule 4; simp; fail)
-     apply (rule 2)
-    by (auto simp: TWL_to_clauses_state_conv_def extract_model_of_state_def
-        state_wl_l_def twl_st_l_def convert_lits_l_map_lit_of)
-  then have IsaSAT_SAT: \<open>(uncurry (\<lambda>_. IsaSAT), uncurry (\<lambda>_. SAT')) \<in>
-     [\<lambda>(_, CS). Multiset.Ball CS distinct_mset \<and>
-      (\<forall>C\<in>#CS. \<forall>L\<in>#C. nat_of_lit L \<le> uint_max)]\<^sub>f
-     Id \<times>\<^sub>r list_mset_rel O \<langle>list_mset_rel\<rangle>mset_rel \<rightarrow> \<langle>\<langle>\<langle>Id\<rangle>list_rel\<rangle> option_rel\<rangle>nres_rel\<close>
-    unfolding SAT' IsaSAT
-    by (auto simp: fref_def)
-  have [simp]: \<open> \<up> (x = map_option rev ac) =  \<up> (ac = map_option rev x)\<close> for x ac
-    by (cases ac; cases x) auto
-  have H: \<open>hr_comp model_stat_assn
-        (Collect (case_prod (\<lambda>(M, stat). (=) (map_option rev M)))) = model_assn\<close>
-    by (auto simp: model_assn_def hr_comp_def model_stat_rel_def ex_assn_pair_split eq_commute
-        intro!: ext)
-  have H: \<open>(uncurry IsaSAT_code, uncurry (\<lambda>_. IsaSAT))
-      \<in> [\<lambda>(_, x). Ball (set x) distinct  \<and> (\<forall>C\<in>set x. \<forall>L\<in>set C. nat_of_lit L \<le> uint_max)]\<^sub>a
-         opts_assn\<^sup>d *\<^sub>a (list_assn (list_assn unat_lit_assn))\<^sup>k \<rightarrow> model_assn\<close>
-    using IsaSAT_code.refine[FCOMP IsaSAT_heur_IsaSAT]
-    unfolding list_assn_list_mset_rel_clauses_l_assn H
-    by auto
-  show ?thesis
-    (is \<open>?c \<in> [?pre]\<^sub>a ?im \<rightarrow> ?f\<close>)
-  proof -
-    have H: \<open>?c \<in>
-       [comp_PRE (Id \<times>\<^sub>f list_mset_rel O \<langle>list_mset_rel\<rangle>mset_rel)
-     (\<lambda>(_, CS). Multiset.Ball CS distinct_mset \<and> (\<forall>C\<in>#CS. \<forall>L\<in>#C. nat_of_lit L \<le> uint_max))
-     (\<lambda>x y. case y of (uu_, x) \<Rightarrow> Ball (set x) distinct \<and> (\<forall>C\<in>set x. \<forall>L\<in>set C. nat_of_lit L \<le> uint_max))
-     (\<lambda>x. nofail
-            (uncurry (\<lambda>_. SAT')
-              x))]\<^sub>a hrp_comp (opts_assn\<^sup>d *\<^sub>a (list_assn (list_assn unat_lit_assn))\<^sup>k)
-                      (Id \<times>\<^sub>f
-                       list_mset_rel O
-                       \<langle>list_mset_rel\<rangle>mset_rel) \<rightarrow> hr_comp model_assn (\<langle>\<langle>nat_lit_lit_rel\<rangle>list_rel\<rangle>option_rel)\<close>
-    (is \<open>_ \<in> [?pre']\<^sub>a ?im' \<rightarrow> ?f'\<close>)
-      using hfref_compI_PRE[OF H IsaSAT_SAT] .
-    have pre: \<open>?pre' x\<close> if \<open>?pre x\<close> for x
-      using that by (auto simp: comp_PRE_def list_mset_rel_def br_def
-          mset_rel_def p2rel_def rel2p_def[abs_def] rel_mset_def
-          list_all2_op_eq_map_right_iff')
-    have im: \<open>?im' = ?im\<close>
-      unfolding prod_hrp_comp hrp_comp_dest hrp_comp_keep
-        list_assn_list_mset_rel_clauses_l_assn by auto
-    have f: \<open>?f' = ?f\<close>
-      by auto
-    show ?thesis
-      apply (rule hfref_weaken_pre[OF ])
-       defer
-      using H unfolding im f apply assumption
-      using pre ..
-  qed
-qed
-
-text \<open>Final correctness theorem:\<close>
-lemmas IsaSAT_code_full_correctness = IsaSAT_code[FCOMP SAT_model_if_satisfiable']
+theorem IsaSAT_full_correctness: \<open>(uncurry IsaSAT_code, uncurry (\<lambda>_. model_if_satisfiable))
+\<in> [\<lambda>(_, a).
+      Multiset.Ball a distinct_mset \<and>
+      (\<forall>C\<in>#a.  \<forall>L\<in>#C. nat_of_lit L  \<le> uint_max)]\<^sub>a opts_assn\<^sup>d *\<^sub>a  clauses_l_assn\<^sup>k \<rightarrow> model_assn\<close>
+  using IsaSAT_code.refine[FCOMP IsaSAT_heur_model_if_sat',
+    unfolded list_assn_list_mset_rel_clauses_l_assn]
+  unfolding model_assn_def
+  apply auto
+  done
 
 end
